equip raw_data_item_match with a fractional permission

src/cbor/CBOR.SteelST.fst
@@ -7,67 +7,97 @@ module CborST = CBOR.SteelST.Raw
 module LPA = LowParse.SteelST.ArrayPtr.IntroElim
 module LPS = LowParse.SteelST.SeqMatch
 module LW = LowParse.SteelST.L2ROutput.IntroElim
+module GR = Steel.ST.GhostReference
 
 let cbor_serialized_payload_t = LPS.byte_array
 let cbor_serialized_footprint_t = LPA.array LPS.byte
 
+let cbor_footprint_t = GR.ref unit
+let dummy_cbor_footprint = magic ()
+
+let prod_perm
+  (p1 p2: perm)
+: Tot perm
+= MkPerm ((let open FStar.Real in ( *. )) p1.v p2.v)
+
 let raw_data_item_match_serialized_prop
+  (p: perm)
+  (fp: cbor_footprint_t)
   (c: cbor)
   (v: Cbor.raw_data_item)
   (a: LPS.byte_array)
   (w: LPS.v CborST.parse_raw_data_item_kind Cbor.raw_data_item)
 : GTot prop
 = match c with
-  | CBOR_Case_Serialized c ->
+  | CBOR_Case_Serialized c fp' ->
     c.cbor_serialized_size == LPA.len (LPS.array_of w) /\
     c.cbor_serialized_payload == a /\
-    c.footprint == LPS.array_of w /\
+    LPS.array_of w == LPA.set_array_perm c.footprint (p `prod_perm` LPA.array_perm c.footprint) /\
+    fp == fp' /\
     w.LPS.contents == v
   | _ -> False
 
 [@@__reduce__]
 let raw_data_item_match_serialized0
+  (p: perm)
   (c: cbor)
   (v: Cbor.raw_data_item)
 : Tot vprop
-= exists_ (fun (a: LPS.byte_array) -> exists_ (fun (w: LPS.v CborST.parse_raw_data_item_kind Cbor.raw_data_item) ->
+= exists_ (fun (a: LPS.byte_array) -> exists_ (fun (w: LPS.v CborST.parse_raw_data_item_kind Cbor.raw_data_item) -> exists_ (fun fp ->
+    GR.pts_to fp p () `star`
     LPS.aparse CborST.parse_raw_data_item a w `star`
     pure (
-      raw_data_item_match_serialized_prop c v a w
+      raw_data_item_match_serialized_prop p fp c v a w
     )
-  ))
+  )))
 
 let raw_data_item_match_simple_value_prop
+  (fp: cbor_footprint_t)
   (c: cbor)
   (v: Cbor.raw_data_item)
 : GTot prop
 = match c with
-  | CBOR_Case_Simple_value c -> v == Cbor.Simple c
+  | CBOR_Case_Simple_value c fp' ->
+    v == Cbor.Simple c /\
+    fp == fp'
   | _ -> False
 
 [@@__reduce__]
 let raw_data_item_match_simple_value0
+  (p: perm)
   (c: cbor)
   (v: Cbor.raw_data_item)
 : Tot vprop
-= pure (raw_data_item_match_simple_value_prop c v)
+= exists_ (fun fp ->
+    GR.pts_to fp p () `star`
+    pure (raw_data_item_match_simple_value_prop fp c v)
+  )
 
 let raw_data_item_match_int_prop
+  (fp: cbor_footprint_t)
   (c: cbor)
   (v: Cbor.raw_data_item)
 : GTot prop
 = match c with
-  | CBOR_Case_Int64 c -> v == Cbor.Int64 c.cbor_int_type c.cbor_int_value
+  | CBOR_Case_Int64 c fp' ->
+    v == Cbor.Int64 c.cbor_int_type c.cbor_int_value /\
+    fp == fp'
   | _ -> False
 
 [@@__reduce__]
 let raw_data_item_match_int0
+  (p: perm)
   (c: cbor)
   (v: Cbor.raw_data_item)
 : Tot vprop
-= pure (raw_data_item_match_int_prop c v)
+= exists_ (fun fp ->
+    GR.pts_to fp p () `star`
+    pure (raw_data_item_match_int_prop fp c v)
+  )
 
 let raw_data_item_match_string_prop
+  (p0: perm)
+  (fp: cbor_footprint_t)
   (c: cbor)
   (v: Cbor.raw_data_item)
   (a: A.array U8.t)
@@ -75,22 +105,25 @@ let raw_data_item_match_string_prop
   (w: Seq.seq U8.t)
 : Tot prop
 = match c with
-  | CBOR_Case_String c ->
+  | CBOR_Case_String c fp' p' ->
     U64.v c.cbor_string_length == Seq.length w /\
     v == Cbor.String c.cbor_string_type w /\
-    c.permission == p /\
+    p == p0 `prod_perm` p' /\
+    fp' == fp /\
     c.cbor_string_payload == a
   | _ -> False
 
 [@@__reduce__]
 let raw_data_item_match_string0
+  (p0: perm)
   (c: cbor)
   (v: Cbor.raw_data_item)
 : Tot vprop
-= exists_ (fun a -> exists_ (fun p -> exists_ (fun w ->
+= exists_ (fun a -> exists_ (fun p -> exists_ (fun w -> exists_ (fun fp ->
+    GR.pts_to fp p0 () `star`
     A.pts_to a p w `star`
-    pure (raw_data_item_match_string_prop c v a p w)
-  )))
+    pure (raw_data_item_match_string_prop p0 fp c v a p w)
+  ))))
 
 unfold
 let raw_data_item_match_tagged_prop
@@ -102,77 +135,86 @@ let raw_data_item_match_tagged_prop
 : Tot prop
 = match v, c with
   | Cbor.Tagged tag v2, CBOR_Case_Tagged c ->
-    c.cbor_tagged_tag == tag /\
+    c.cbor_tagged0_tag == tag /\
     Ghost.reveal c.footprint == c' /\
     v2 == v' /\
-    c.cbor_tagged_payload == a
+    c.cbor_tagged0_payload == a
   | _ -> False
 
 [@@__reduce__]
 let raw_data_item_match_tagged0
+  (p: perm)
   (c: cbor)
   (v: Cbor.raw_data_item)
   (raw_data_item_match: (cbor -> (v': Cbor.raw_data_item { v' << v }) -> vprop))
 : Tot vprop
 = exists_ (fun a -> exists_ (fun c' -> exists_ (fun v' ->
-    R.pts_to a full_perm c' `star`
+    R.pts_to a p c' `star`
     raw_data_item_match c' v' `star`
     pure (raw_data_item_match_tagged_prop c v a c' v')
   )))
 
 let raw_data_item_match_array_prop
+  (fp: cbor_footprint_t)
   (c: cbor)
   (v: Cbor.raw_data_item)
   (s: Seq.seq cbor)
   (a: A.array cbor)
 : GTot prop
 = match c, v with
-  | CBOR_Case_Array c, Cbor.Array l ->
+  | CBOR_Case_Array c fp', Cbor.Array l ->
     U64.v c.cbor_array_length == List.Tot.length l /\
     Ghost.reveal c.footprint == s /\
+    fp' == fp /\
     c.cbor_array_payload == a
   | _ -> False
 
 [@@__reduce__]
 let raw_data_item_match_array0
+  (p: perm)
   (c: cbor)
   (v: Cbor.raw_data_item { Cbor.Array? v })
   (raw_data_item_array_match: (Seq.seq cbor -> (v': list Cbor.raw_data_item { v' << v }) -> vprop))
 : Tot vprop
-= exists_ (fun (a: A.array cbor) -> exists_ (fun (c': Seq.seq cbor) ->
-    A.pts_to a full_perm c' `star`
+= exists_ (fun (a: A.array cbor) -> exists_ (fun (c': Seq.seq cbor) -> exists_ (fun fp ->
+    GR.pts_to fp p () `star`
+    A.pts_to a p c' `star`
     raw_data_item_array_match c' (Cbor.Array?.v v) `star`
     pure (
-      raw_data_item_match_array_prop c v c' a
+      raw_data_item_match_array_prop fp c v c' a
     )
-  ))
+  )))
 
 let raw_data_item_match_map_prop
+  (fp: cbor_footprint_t)
   (c: cbor)
   (v: Cbor.raw_data_item)
   (a: A.array cbor_map_entry)
   (s: Seq.seq cbor_map_entry)
 : GTot prop
 = match c, v with
-  | CBOR_Case_Map c, Cbor.Map l ->
+  | CBOR_Case_Map c fp', Cbor.Map l ->
     U64.v c.cbor_map_length == List.Tot.length l /\
     Ghost.reveal c.footprint == s /\
+    fp' == fp /\
     c.cbor_map_payload == a
   | _ -> False
 
 [@@__reduce__]
 let raw_data_item_match_map0
+  (p: perm)
   (c: cbor)
   (v: Cbor.raw_data_item { Cbor.Map? v })
   (raw_data_item_map_match: (Seq.seq cbor_map_entry -> (v': list (Cbor.raw_data_item & Cbor.raw_data_item) { v' << v }) -> vprop))
 : Tot vprop
-= exists_ (fun (a: A.array cbor_map_entry) -> exists_ (fun (c': Seq.seq cbor_map_entry) ->
-    A.pts_to a full_perm c' `star`
+= exists_ (fun (a: A.array cbor_map_entry) -> exists_ (fun (c': Seq.seq cbor_map_entry) -> exists_ (fun fp ->
+    GR.pts_to fp p () `star`
+    A.pts_to a p c' `star`
     raw_data_item_map_match c' (Cbor.Map?.v v) `star`
     pure (
-      raw_data_item_match_map_prop c v a c'
+      raw_data_item_match_map_prop fp c v a c'
     )
-  ))
+  )))
 
 let raw_data_item_map_entry_match'
   (l: list (Cbor.raw_data_item & Cbor.raw_data_item))
@@ -183,105 +225,287 @@ let raw_data_item_map_entry_match'
 = raw_data_item_map_entry_match1 c1 v1 raw_data_item_match
 
 let rec raw_data_item_match
+  (p: perm)
   (c: cbor)
   (v: Cbor.raw_data_item)
 : Tot vprop
   (decreases v)
 = match c, v with
-  | CBOR_Case_Serialized _, _ -> raw_data_item_match_serialized0 c v
-  | CBOR_Case_Simple_value _, Cbor.Simple _ -> raw_data_item_match_simple_value0 c v
-  | CBOR_Case_Int64 _, Cbor.Int64 _ _ -> raw_data_item_match_int0 c v
-  | CBOR_Case_String _, Cbor.String _ _ -> raw_data_item_match_string0 c v
-  | CBOR_Case_Array _, Cbor.Array _ -> raw_data_item_match_array0 c v raw_data_item_array_match'
-  | CBOR_Case_Map _, Cbor.Map _ -> raw_data_item_match_map0 c v raw_data_item_map_match'
-  | CBOR_Case_Tagged _, Cbor.Tagged _ _ -> raw_data_item_match_tagged0 c v raw_data_item_match
+  | CBOR_Case_Serialized _ _, _ -> raw_data_item_match_serialized0 p c v
+  | CBOR_Case_Simple_value _ _, Cbor.Simple _ -> raw_data_item_match_simple_value0 p c v
+  | CBOR_Case_Int64 _ _, Cbor.Int64 _ _ -> raw_data_item_match_int0 p c v
+  | CBOR_Case_String _ _ _, Cbor.String _ _ -> raw_data_item_match_string0 p c v
+  | CBOR_Case_Array _ _, Cbor.Array _ -> raw_data_item_match_array0 p c v (raw_data_item_array_match' p)
+  | CBOR_Case_Map _ _, Cbor.Map _ -> raw_data_item_match_map0 p c v (raw_data_item_map_match' p)
+  | CBOR_Case_Tagged _, Cbor.Tagged _ _ -> raw_data_item_match_tagged0 p c v (raw_data_item_match p)
   | _ -> pure False
 
 and raw_data_item_array_match'
+  (p: perm)
   (c: Seq.seq cbor)
   (v: list Cbor.raw_data_item)
 : Tot vprop
   (decreases v)
-= LPS.seq_list_match c v raw_data_item_match
+= LPS.seq_list_match c v (raw_data_item_match p)
 
 and raw_data_item_map_match'
+  (p: perm)
   (c: Seq.seq cbor_map_entry)
   (v: list (Cbor.raw_data_item & Cbor.raw_data_item))
 : Tot vprop
   (decreases v)
-= LPS.seq_list_match c v (raw_data_item_map_entry_match' v raw_data_item_match)
+= LPS.seq_list_match c v (raw_data_item_map_entry_match' v (raw_data_item_match p))
 
 #set-options "--ide_id_info_off"
 
 let raw_data_item_match_get_case
   (#opened: _)
+  (#p: perm)
   (#v: Cbor.raw_data_item)
   (c: cbor)
 : STGhost unit opened
-    (raw_data_item_match c v)
-    (fun _ -> raw_data_item_match c v)
+    (raw_data_item_match p c v)
+    (fun _ -> raw_data_item_match p c v)
     True
     (fun _ -> match c, v with
-    | CBOR_Case_Serialized _, _
-    | CBOR_Case_Array _, Cbor.Array _
-    | CBOR_Case_Int64 _, Cbor.Int64 _ _
-    | CBOR_Case_Map _, Cbor.Map _
-    | CBOR_Case_Simple_value _, Cbor.Simple _
-    | CBOR_Case_String _, Cbor.String _ _
+    | CBOR_Case_Serialized _ _, _
+    | CBOR_Case_Array _ _, Cbor.Array _
+    | CBOR_Case_Int64 _ _, Cbor.Int64 _ _
+    | CBOR_Case_Map _ _, Cbor.Map _
+    | CBOR_Case_Simple_value _ _, Cbor.Simple _
+    | CBOR_Case_String _ _ _, Cbor.String _ _
     | CBOR_Case_Tagged _, Cbor.Tagged _ _
       -> True
     | _ -> False
     )
 = match c, v with
-    | CBOR_Case_Serialized _, _
-    | CBOR_Case_Array _, Cbor.Array _
-    | CBOR_Case_Int64 _, Cbor.Int64 _ _
-    | CBOR_Case_Map _, Cbor.Map _
-    | CBOR_Case_Simple_value _, Cbor.Simple _
-    | CBOR_Case_String _, Cbor.String _ _
+    | CBOR_Case_Serialized _ _, _
+    | CBOR_Case_Array _ _, Cbor.Array _
+    | CBOR_Case_Int64 _ _, Cbor.Int64 _ _
+    | CBOR_Case_Map _ _, Cbor.Map _
+    | CBOR_Case_Simple_value _ _, Cbor.Simple _
+    | CBOR_Case_String _ _ _, Cbor.String _ _
     | CBOR_Case_Tagged _, Cbor.Tagged _ _
       -> noop ()
     | _ ->
-      rewrite (raw_data_item_match c v) (pure False);
+      rewrite (raw_data_item_match p c v) (pure False);
       let _ = gen_elim () in
-      rewrite emp (raw_data_item_match c v)
+      rewrite emp (raw_data_item_match p c v)
+
+assume
+val ref_pts_to_perm (#a: _) (#u: _) (#p: _) (#v: _) (r: R.ref a)
+  : STGhost unit u
+      (R.pts_to r p v)
+      (fun _ -> R.pts_to r p v)
+      True
+      (fun _ -> p `lesser_equal_perm` full_perm)
+
+let raw_data_item_match_perm_le_full_perm
+  (#opened: _)
+  (#p: perm)
+  (#v: Cbor.raw_data_item)
+  (c: cbor)
+: STGhost unit opened
+    (raw_data_item_match p c v)
+    (fun _ -> raw_data_item_match p c v)
+    True
+    (fun _ -> p `lesser_equal_perm` full_perm)
+= match c, v with
+    | CBOR_Case_Serialized _ _, _ ->
+      rewrite
+        (raw_data_item_match p c v)
+        (raw_data_item_match_serialized0 p c v);
+      let _ = gen_elim () in
+      GR.pts_to_perm _;
+      rewrite 
+        (raw_data_item_match_serialized0 p c v)
+        (raw_data_item_match p c v)
+    | CBOR_Case_Int64 _ _, Cbor.Int64 _ _ ->
+      rewrite
+        (raw_data_item_match p c v)
+        (raw_data_item_match_int0 p c v);
+      let _ = gen_elim () in
+      GR.pts_to_perm _;
+      rewrite
+        (raw_data_item_match_int0 p c v)
+        (raw_data_item_match p c v)
+    | CBOR_Case_Simple_value _ _, Cbor.Simple _ ->
+      rewrite
+        (raw_data_item_match p c v)
+        (raw_data_item_match_simple_value0 p c v);
+      let _ = gen_elim () in
+      GR.pts_to_perm _;
+      rewrite
+        (raw_data_item_match_simple_value0 p c v)
+        (raw_data_item_match p c v)
+    | CBOR_Case_String _ _ _, Cbor.String _ _ ->
+      rewrite
+        (raw_data_item_match p c v)
+        (raw_data_item_match_string0 p c v);
+      let _ = gen_elim () in
+      GR.pts_to_perm _;
+      rewrite
+        (raw_data_item_match_string0 p c v)
+        (raw_data_item_match p c v)
+    | CBOR_Case_Array a sfp, Cbor.Array v0 ->
+      assert_norm (
+        raw_data_item_match p (CBOR_Case_Array a sfp) (Cbor.Array v0) ==
+          raw_data_item_match_array0 p (CBOR_Case_Array a sfp) (Cbor.Array v0) (raw_data_item_array_match' p)
+      );
+      rewrite
+        (raw_data_item_match p c v)
+        (raw_data_item_match_array0 p c v (raw_data_item_array_match' p));
+      let _ = gen_elim () in
+      GR.pts_to_perm _;
+      rewrite
+        (raw_data_item_match_array0 p c v (raw_data_item_array_match' p))
+        (raw_data_item_match p c v)
+    | CBOR_Case_Map a sfp, Cbor.Map v0 ->
+      assert_norm (
+        raw_data_item_match p (CBOR_Case_Map a sfp) (Cbor.Map v0) ==
+          raw_data_item_match_map0 p (CBOR_Case_Map a sfp) (Cbor.Map v0) (raw_data_item_map_match' p)
+      );
+      rewrite
+        (raw_data_item_match p c v)
+        (raw_data_item_match_map0 p c v (raw_data_item_map_match' p));
+      let _ = gen_elim () in
+      GR.pts_to_perm _;
+      rewrite
+        (raw_data_item_match_map0 p c v (raw_data_item_map_match' p))
+        (raw_data_item_match p c v)
+    | CBOR_Case_Tagged a, Cbor.Tagged tg v0 ->
+      assert_norm (
+        raw_data_item_match p (CBOR_Case_Tagged a) (Cbor.Tagged tg v0) ==
+          raw_data_item_match_tagged0 p (CBOR_Case_Tagged a) (Cbor.Tagged tg v0) (raw_data_item_match p)
+      );
+      rewrite
+        (raw_data_item_match p c v)
+        (raw_data_item_match_tagged0 p c v (raw_data_item_match p));
+      let _ = gen_elim () in
+      ref_pts_to_perm _;
+      rewrite
+        (raw_data_item_match_tagged0 p c v (raw_data_item_match p))
+        (raw_data_item_match p c v)
+    | _ ->
+      rewrite
+        (raw_data_item_match p c v)
+        (pure False);
+      let _ = gen_elim () in
+      rewrite // by contradiction
+        emp
+        (raw_data_item_match p c v)
+
+let diff_perm
+  (high low: perm)
+: Pure perm
+  (requires (
+    low `lesser_equal_perm` high /\
+    (~ (low == high))
+  ))
+  (ensures (fun diff ->
+    high == low `sum_perm` diff
+  ))
+= MkPerm ((let open FStar.Real in ( -. )) high.v low.v)
+
+assume
+val gref_share_gen
+  (#t: Type)
+  (#opened: _)
+  (#p: perm)
+  (#v: t)
+  (r: GR.ref t)
+  (p1 p2: perm)
+: STGhost unit opened
+    (GR.pts_to r p v)
+    (fun _ -> GR.pts_to r p1 v `star` GR.pts_to r p2 v)
+    (p == p1 `sum_perm` p2)
+    (fun _ -> True)
+
+let gref_lower_perm
+  (#t: Type)
+  (#opened: _)
+  (#high: perm)
+  (#v: t)
+  (r: GR.ref t)
+  (low: perm)
+: STGhost unit opened
+    (GR.pts_to r high v)
+    (fun _ -> GR.pts_to r low v `star`
+      (GR.pts_to r low v `implies_` GR.pts_to r high v)
+    )
+    (low `lesser_equal_perm` high)
+    (fun _ -> True)
+= if FStar.StrongExcludedMiddle.strong_excluded_middle (low == high)
+  then
+    vpattern_rewrite_with_implies
+      (fun p -> GR.pts_to _ p _)
+      low
+  else begin
+    let diff = diff_perm high low in
+    gref_share_gen r low diff;
+    intro_implies
+      (GR.pts_to r low v)
+      (GR.pts_to r high v)
+      (GR.pts_to r diff v)
+      (fun _ ->
+        GR.gather #_ #_ #low r;
+        vpattern_rewrite (fun p -> GR.pts_to _ p _) high
+      )
+  end
+
+let div_perm
+  (a b: perm)
+: Pure perm
+    (requires True)
+    (ensures (fun q ->
+      a == b `prod_perm` q
+    ))
+= MkPerm ((let open FStar.Real in ( /. )) a.v b.v)
 
 let read_valid_cbor_from_buffer_with_size_strong
   (#va: LPS.v CborST.parse_raw_data_item_kind Cbor.raw_data_item)
+  (p: perm)
   (a: LPS.byte_array)
   (alen: SZ.t)
 : ST cbor
     (LPS.aparse CborST.parse_raw_data_item a va)
     (fun c' ->
-      raw_data_item_match c' va.contents `star`
-      (raw_data_item_match c' va.contents `implies_` LPS.aparse CborST.parse_raw_data_item a va)
+      raw_data_item_match p c' va.contents `star`
+      (raw_data_item_match p c' va.contents `implies_` LPS.aparse CborST.parse_raw_data_item a va)
     )
-    (alen == LPA.len (LPS.array_of va))
+    (alen == LPA.len (LPS.array_of va) /\
+      p `lesser_equal_perm` full_perm
+    )
     (fun c' -> CBOR_Case_Serialized? c')
 = [@@inline_let]
   let c_pl : cbor_serialized = ({
     cbor_serialized_size = alen;
     cbor_serialized_payload = a;
-    footprint = LPS.array_of va;
+    footprint = LPA.set_array_perm (LPS.array_of va) (div_perm (LPA.array_perm (LPS.array_of va)) p);
   })
   in
+  let fp = GR.alloc () in
+  gref_lower_perm fp p;
   [@@inline_let]
-  let c' = CBOR_Case_Serialized c_pl in
+  let c' = CBOR_Case_Serialized c_pl fp in
   noop ();
   rewrite_with_implies
-    (raw_data_item_match_serialized0 (CBOR_Case_Serialized c_pl) va.contents)
-    (raw_data_item_match c' va.contents);
+    (raw_data_item_match_serialized0 p (CBOR_Case_Serialized c_pl fp) va.contents)
+    (raw_data_item_match p c' va.contents);
   intro_implies
-    (raw_data_item_match_serialized0 (CBOR_Case_Serialized c_pl) va.contents)
+    (raw_data_item_match_serialized0 p (CBOR_Case_Serialized c_pl fp) va.contents)
     (LPS.aparse CborST.parse_raw_data_item a va)
-    emp
+    (GR.pts_to fp p () `implies_` GR.pts_to fp full_perm ())
     (fun _ ->
       let _ = gen_elim () in
+      rewrite (GR.pts_to _ _ _) (GR.pts_to fp p ());
+      elim_implies (GR.pts_to _ _ _) (GR.pts_to _ _ _);
+      GR.free _;
       rewrite (LPS.aparse CborST.parse_raw_data_item _ _) (LPS.aparse CborST.parse_raw_data_item a va) // works thanks to c_pl.footprint
     );
   implies_trans
-    (raw_data_item_match c' va.contents)
-    (raw_data_item_match_serialized0 (CBOR_Case_Serialized c_pl) va.contents)
+    (raw_data_item_match p c' va.contents)
+    (raw_data_item_match_serialized0 p (CBOR_Case_Serialized c_pl fp) va.contents)
     (LPS.aparse CborST.parse_raw_data_item a va);
   return c'
 
@@ -292,11 +516,11 @@ let read_valid_cbor_from_buffer_with_size
 : ST cbor
     (LPS.aparse CborST.parse_raw_data_item a va)
     (fun c' ->
-      raw_data_item_match c' va.contents
+      raw_data_item_match full_perm c' va.contents
     )
     (alen == LPA.len (LPS.array_of va))
     (fun c' -> CBOR_Case_Serialized? c')
-= let c' = read_valid_cbor_from_buffer_with_size_strong a alen in
+= let c' = read_valid_cbor_from_buffer_with_size_strong full_perm a alen in
   drop (_ `implies_` _);
   return c'
 
@@ -306,20 +530,21 @@ let read_valid_cbor_from_buffer
 : STT cbor
     (LPS.aparse CborST.parse_raw_data_item a va)
     (fun c' ->
-      raw_data_item_match c' va.contents
+      raw_data_item_match full_perm c' va.contents
     )
 = let alen = LPS.get_parsed_size CborST.jump_raw_data_item a in
   read_valid_cbor_from_buffer_with_size a alen
 
 let destr_cbor_serialized
+  (#p: perm)
   (#va: Ghost.erased Cbor.raw_data_item)
   (c: cbor)
 : ST cbor_serialized
-    (raw_data_item_match c va)
+    (raw_data_item_match p c va)
     (fun c' -> exists_ (fun vc ->
       LPS.aparse CborST.parse_raw_data_item c'.cbor_serialized_payload vc `star`
       (LPS.aparse CborST.parse_raw_data_item c'.cbor_serialized_payload vc `implies_`
-        raw_data_item_match c va
+        raw_data_item_match p c va
       ) `star`
       pure (
         vc.LPS.contents == Ghost.reveal va /\
@@ -327,24 +552,25 @@ let destr_cbor_serialized
     )))
     (CBOR_Case_Serialized? c)
     (fun _ -> True)
-= let CBOR_Case_Serialized c' = c in
+= let CBOR_Case_Serialized c' fp = c in
   rewrite_with_implies
-    (raw_data_item_match c va)
-    (raw_data_item_match_serialized0 (CBOR_Case_Serialized c') va);
+    (raw_data_item_match p c va)
+    (raw_data_item_match_serialized0 p (CBOR_Case_Serialized c' fp) va);
   let _ = gen_elim () in
+  rewrite (GR.pts_to _ _ _) (GR.pts_to fp p ());
   let vc = vpattern_replace (LPS.aparse CborST.parse_raw_data_item _) in
   vpattern_rewrite (fun a -> LPS.aparse CborST.parse_raw_data_item a _) c'.cbor_serialized_payload;
   intro_implies
     (LPS.aparse CborST.parse_raw_data_item c'.cbor_serialized_payload vc)
-    (raw_data_item_match_serialized0 (CBOR_Case_Serialized c') va)
-    emp
+    (raw_data_item_match_serialized0 p (CBOR_Case_Serialized c' fp) va)
+    (GR.pts_to fp p ())
     (fun _ ->
       noop (); noop () // FIXME: WHY WHY WHY do I need an explicit bind here?
     );
   implies_trans
     (LPS.aparse CborST.parse_raw_data_item c'.cbor_serialized_payload vc)
-    (raw_data_item_match_serialized0 (CBOR_Case_Serialized c') va)
-    (raw_data_item_match c va);
+    (raw_data_item_match_serialized0 p (CBOR_Case_Serialized c' fp) va)
+    (raw_data_item_match p c va);
   return c'
 
 let serialize_cbor_error
@@ -420,9 +646,9 @@ let read_cbor'
         (A.pts_to rem p _)
         (LPA.arrayptr rem' _)
         (A.pts_to a p va);
-      let c = read_valid_cbor_from_buffer_with_size_strong a' sz' in
+      let c = read_valid_cbor_from_buffer_with_size_strong full_perm a' sz' in
       implies_trans_l1
-        (raw_data_item_match c _)
+        (raw_data_item_match full_perm c _)
         (LPS.aparse CborST.parse_raw_data_item a' _)
         (A.pts_to rem p _)
         (A.pts_to a p va);
@@ -434,18 +660,18 @@ let read_cbor'
       }
       in
       vpattern_rewrite_with_implies
-        (fun c -> raw_data_item_match c _)
+        (fun c -> raw_data_item_match full_perm c _)
         res.read_cbor_payload;
       implies_trans_l1
-        (raw_data_item_match res.read_cbor_payload _)
-        (raw_data_item_match c _)
+        (raw_data_item_match full_perm res.read_cbor_payload _)
+        (raw_data_item_match full_perm c _)
         (A.pts_to rem p _)
         (A.pts_to a p va);
       vpattern_rewrite_with_implies
         (fun rem -> A.pts_to rem p _)
         res.read_cbor_remainder;
       implies_trans_r1
-        (raw_data_item_match res.read_cbor_payload _)
+        (raw_data_item_match full_perm res.read_cbor_payload _)
         (A.pts_to res.read_cbor_remainder _ _)
         (A.pts_to rem _ _)
         (A.pts_to a p va);
@@ -517,7 +743,7 @@ let read_deterministically_encoded_cbor
     in
     elim_implies
       (LPS.aparse CborST.parse_raw_data_item _ _)
-      (raw_data_item_match _ _);
+      (raw_data_item_match full_perm _ _);
     if test
     then begin
       noop ();
@@ -527,11 +753,11 @@ let read_deterministically_encoded_cbor
         (read_deterministically_encoded_cbor_post a p va res);
       return res
     end else begin
-      let v = vpattern_erased (raw_data_item_match _) in
+      let v = vpattern_erased (raw_data_item_match full_perm _) in
       let rem = vpattern_erased (A.pts_to _ _) in
       serialize_deterministically_encoded_cbor_error va r v rem;
       elim_implies
-        (raw_data_item_match _ _ `star` A.pts_to _ _ _)
+        (raw_data_item_match full_perm _ _ `star` A.pts_to _ _ _)
         (A.pts_to a p va);
       rewrite
         (read_deterministically_encoded_cbor_error_post a p va)
@@ -546,14 +772,15 @@ let cbor_size_comp_for
   (va: Ghost.erased Cbor.raw_data_item)
   (c: cbor)
 : Tot Type
-= (sz: SZ.t) ->
+= (#p: perm) ->
+  (sz: SZ.t) ->
   (perr: R.ref bool) ->
   STT SZ.t
-    (raw_data_item_match c (Ghost.reveal va) `star`
+    (raw_data_item_match p c (Ghost.reveal va) `star`
       R.pts_to perr full_perm false
     )
     (fun res ->
-      raw_data_item_match c (Ghost.reveal va) `star`
+      raw_data_item_match p c (Ghost.reveal va) `star`
       exists_ (fun err ->
         R.pts_to perr full_perm err `star`
         pure (LowParse.SteelST.Write.size_comp_for_post CborST.serialize_raw_data_item va sz res err)
@@ -573,6 +800,7 @@ let l2r_write_cbor_post
 
 [@@__reduce__]
 let cbor_l2r_writer_for_post
+  (p: perm)
   (va: Ghost.erased Cbor.raw_data_item)
   (c: cbor)
   (vout: LPA.array LPS.byte)
@@ -582,7 +810,7 @@ let cbor_l2r_writer_for_post
   (vout': LPA.array LPS.byte)
 : Tot vprop
 =
-  raw_data_item_match c (Ghost.reveal va) `star`
+  raw_data_item_match p c (Ghost.reveal va) `star`
   LPS.aparse CborST.parse_raw_data_item res vres `star`
   LW.vp out vout' `star`
   pure (
@@ -595,14 +823,15 @@ let cbor_l2r_writer_for
   (va: Ghost.erased Cbor.raw_data_item)
   (c: cbor)
 : Tot Type
-= (#vout: LPA.array LPS.byte) ->
+= (#p: perm) ->
+  (#vout: LPA.array LPS.byte) ->
   (out: LW.t) ->
   ST LPS.byte_array
-    (raw_data_item_match c (Ghost.reveal va) `star`
+    (raw_data_item_match p c (Ghost.reveal va) `star`
       LW.vp out vout
     )
     (fun res -> exists_ (fun (vres: LPS.v CborST.parse_raw_data_item_kind Cbor.raw_data_item) -> exists_ (fun (vout': LPA.array LPS.byte) ->
-      cbor_l2r_writer_for_post va c vout out res vres vout'
+      cbor_l2r_writer_for_post p va c vout out res vres vout'
     )))
     (Seq.length (LPS.serialize CborST.serialize_raw_data_item va) <= LPA.length vout)
     (fun _ -> True)
@@ -611,13 +840,13 @@ let size_comp_for_serialized
   (#va: Ghost.erased Cbor.raw_data_item)
   (c: cbor {CBOR_Case_Serialized? c})
 : Tot (cbor_size_comp_for va c)
-= fun sz perr ->
+= fun #p sz perr ->
     let c' = destr_cbor_serialized c in
     let _ = gen_elim () in
     LPS.aparse_serialized_length CborST.serialize_raw_data_item _;
     elim_implies
       (LPS.aparse CborST.parse_raw_data_item _ _)
-      (raw_data_item_match _ _);
+      (raw_data_item_match p _ _);
     if c'.cbor_serialized_size `SZ.gt` sz
     then begin
       noop ();
@@ -634,7 +863,7 @@ let l2r_writer_for_serialized
   (#va: Ghost.erased Cbor.raw_data_item)
   (c: cbor {CBOR_Case_Serialized? c})
 : Tot (cbor_l2r_writer_for va c)
-= fun #vout out ->
+= fun #p #vout out ->
     let c' = destr_cbor_serialized c in
     let _ = gen_elim () in
     LPS.aparse_serialized_length CborST.serialize_raw_data_item _;
@@ -642,7 +871,7 @@ let l2r_writer_for_serialized
     implies_trans
       (LPA.arrayptr c'.cbor_serialized_payload _)
       (LPS.aparse CborST.parse_raw_data_item _ _)
-      (raw_data_item_match _ _);
+      (raw_data_item_match p _ _);
     let res = LW.split out c'.cbor_serialized_size in
     let _ = gen_elim () in
     let vout' = vpattern_replace (LW.vp out) in
@@ -650,27 +879,27 @@ let l2r_writer_for_serialized
     let vres = LPS.intro_aparse CborST.parse_raw_data_item res in
     elim_implies
       (LPA.arrayptr c'.cbor_serialized_payload _)
-      (raw_data_item_match _ _);
-    assert_ (cbor_l2r_writer_for_post va c vout out res vres vout'); // FIXME: WHY WHY WHY?
+      (raw_data_item_match p _ _);
+    assert_ (cbor_l2r_writer_for_post p va c vout out res vres vout'); // FIXME: WHY WHY WHY?
     return res
 
 let destr_cbor_int64
-  #va c
+  #p #va c
 = raw_data_item_match_get_case c;
   match c with
-  | CBOR_Case_Int64 c' ->
+  | CBOR_Case_Int64 c' fp ->
     rewrite_with_implies
-      (raw_data_item_match c (Ghost.reveal va))
-      (raw_data_item_match_int0 c (Ghost.reveal va));
+      (raw_data_item_match p c (Ghost.reveal va))
+      (raw_data_item_match_int0 p c (Ghost.reveal va));
     let _ = gen_elim () in
     elim_implies
-      (raw_data_item_match_int0 c (Ghost.reveal va))
-      (raw_data_item_match c (Ghost.reveal va));
+      (raw_data_item_match_int0 p c (Ghost.reveal va))
+      (raw_data_item_match p c (Ghost.reveal va));
     return c'
-  | CBOR_Case_Serialized cs ->
+  | CBOR_Case_Serialized cs fp ->
     rewrite_with_implies
-      (raw_data_item_match c (Ghost.reveal va))
-      (raw_data_item_match_serialized0 c (Ghost.reveal va));
+      (raw_data_item_match p c (Ghost.reveal va))
+      (raw_data_item_match_serialized0 p c (Ghost.reveal va));
     let _ = gen_elim () in
     vpattern_rewrite (fun a -> LPS.aparse CborST.parse_raw_data_item a _) cs.cbor_serialized_payload;
     let typ = CborST.read_major_type cs.cbor_serialized_payload in
@@ -682,8 +911,8 @@ let destr_cbor_int64
     in
     noop ();
     elim_implies
-      (raw_data_item_match_serialized0 c (Ghost.reveal va))
-      (raw_data_item_match c (Ghost.reveal va));
+      (raw_data_item_match_serialized0 p c (Ghost.reveal va))
+      (raw_data_item_match p c (Ghost.reveal va));
     return c'
 
 let size_comp_for_int64
@@ -707,44 +936,39 @@ let l2r_writer_for_int64
     return res
 
 let constr_cbor_int64
-  (ty: Cbor.major_type_uint64_or_neg_int64)
-  (value: U64.t)
-: ST cbor
-    emp
-    (fun c -> raw_data_item_match c (Cbor.Int64 ty value))
-    True
-    (fun c -> c == CBOR_Case_Int64 ({ cbor_int_type = ty; cbor_int_value = value }))
-= [@@inline_let]
-  let c = CBOR_Case_Int64 ({ cbor_int_type = ty; cbor_int_value = value }) in
+  ty value
+= let fp = GR.alloc () in
+  [@@inline_let]
+  let c = CBOR_Case_Int64 ({ cbor_int_type = ty; cbor_int_value = value }) fp in
   noop ();
   rewrite
-    (raw_data_item_match_int0 c (Cbor.Int64 ty value))
-    (raw_data_item_match c (Cbor.Int64 ty value));
+    (raw_data_item_match_int0 full_perm c (Cbor.Int64 ty value))
+    (raw_data_item_match full_perm c (Cbor.Int64 ty value));
   return c
 
 let destr_cbor_simple_value
-  #va c
+  #p #va c
 = raw_data_item_match_get_case c;
   match c with
-  | CBOR_Case_Simple_value c' ->
+  | CBOR_Case_Simple_value c' _ ->
     rewrite_with_implies
-      (raw_data_item_match c (Ghost.reveal va))
-      (raw_data_item_match_simple_value0 c (Ghost.reveal va));
+      (raw_data_item_match p c (Ghost.reveal va))
+      (raw_data_item_match_simple_value0 p c (Ghost.reveal va));
     let _ = gen_elim () in
     elim_implies
-      (raw_data_item_match_simple_value0 c (Ghost.reveal va))
-      (raw_data_item_match c (Ghost.reveal va));
+      (raw_data_item_match_simple_value0 p c (Ghost.reveal va))
+      (raw_data_item_match p c (Ghost.reveal va));
     return c'
-  | CBOR_Case_Serialized cs ->
+  | CBOR_Case_Serialized cs _ ->
     rewrite_with_implies
-      (raw_data_item_match c (Ghost.reveal va))
-      (raw_data_item_match_serialized0 c (Ghost.reveal va));
+      (raw_data_item_match p c (Ghost.reveal va))
+      (raw_data_item_match_serialized0 p c (Ghost.reveal va));
     let _ = gen_elim () in
     vpattern_rewrite (fun a -> LPS.aparse CborST.parse_raw_data_item a _) cs.cbor_serialized_payload;
     let c' = CborST.read_simple_value cs.cbor_serialized_payload in
     elim_implies
-      (raw_data_item_match_serialized0 c (Ghost.reveal va))
-      (raw_data_item_match c (Ghost.reveal va));
+      (raw_data_item_match_serialized0 p c (Ghost.reveal va))
+      (raw_data_item_match p c (Ghost.reveal va));
     return c'
 
 let size_comp_for_simple_value
@@ -768,136 +992,73 @@ let l2r_writer_for_simple_value
     return res
 
 let constr_cbor_simple_value
-  (value: Cbor.simple_value)
-: ST cbor
-    emp
-    (fun c -> raw_data_item_match c (Cbor.Simple value))
-    True
-    (fun c -> c == CBOR_Case_Simple_value value)
-= [@@inline_let]
-  let c = CBOR_Case_Simple_value value in
+  value
+= let fp = GR.alloc () in
+  [@@inline_let]
+  let c = CBOR_Case_Simple_value value fp in
   noop ();
   rewrite
-    (raw_data_item_match_simple_value0 c (Cbor.Simple value))
-    (raw_data_item_match c (Cbor.Simple value));
+    (raw_data_item_match_simple_value0 full_perm c (Cbor.Simple value))
+    (raw_data_item_match full_perm c (Cbor.Simple value));
   return c
 
-let destr_cbor_string'
-  (#va: Ghost.erased Cbor.raw_data_item)
-  (c: cbor)
-: ST cbor_string
-    (raw_data_item_match c (Ghost.reveal va))
-    (fun c' ->
-      raw_data_item_match (CBOR_Case_String c') (Ghost.reveal va) `star`
-      (raw_data_item_match (CBOR_Case_String c') (Ghost.reveal va) `implies_` raw_data_item_match c (Ghost.reveal va))
-    )
-    (Cbor.String? (Ghost.reveal va))
-    (fun _ -> True)
+let destr_cbor_string
+  #p #va c
 = raw_data_item_match_get_case c;
   match c with
-  | CBOR_Case_String c' ->
+  | CBOR_Case_String c' fp p' ->
     rewrite_with_implies
-      (raw_data_item_match c (Ghost.reveal va))
-      (raw_data_item_match (CBOR_Case_String c') (Ghost.reveal va));
-    return c'
-  | CBOR_Case_Serialized cs ->
-    rewrite_with_implies
-      (raw_data_item_match c (Ghost.reveal va))
-      (raw_data_item_match_serialized0 c (Ghost.reveal va));
+      (raw_data_item_match p c (Ghost.reveal va))
+      (raw_data_item_match_string0 p c (Ghost.reveal va));
     let _ = gen_elim () in
-    vpattern_rewrite (fun a -> LPS.aparse CborST.parse_raw_data_item a _) cs.cbor_serialized_payload;
-    let va' = vpattern_replace (LPS.aparse CborST.parse_raw_data_item _) in
+    let vc' = vpattern_erased (A.pts_to _ _) in
+    let np = p `prod_perm` p' in
+    rewrite (A.pts_to _ _ _) (A.pts_to c'.cbor_string_payload np vc');
+    intro_implies
+      (A.pts_to c'.cbor_string_payload np vc')
+      (raw_data_item_match_string0 p c (Ghost.reveal va))
+      (GR.pts_to _ _ _)
+      (fun _ ->
+        noop ();
+        noop ()
+      );
+    implies_trans
+      (A.pts_to c'.cbor_string_payload np vc')
+      (raw_data_item_match_string0 p c (Ghost.reveal va))
+      (raw_data_item_match p c (Ghost.reveal va));
+    return c'
+  | _ ->
+    let cs = destr_cbor_serialized c in
+    let _ = gen_elim () in
     let typ = CborST.read_major_type cs.cbor_serialized_payload in
     let len = CborST.read_argument_as_uint64 cs.cbor_serialized_payload in
     let lpayload = CborST.focus_string cs.cbor_serialized_payload in
     let _ = gen_elim () in
+    implies_trans
+      (LPA.arrayptr _ _)
+      (LPS.aparse CborST.parse_raw_data_item _ _)
+      (raw_data_item_match _ _ _);
     let payload = LPA.elim_arrayptr_with_implies lpayload in
     let _ = gen_elim () in
     implies_trans
       (A.pts_to _ _ _)
       (LPA.arrayptr _ _)
-      (LPS.aparse CborST.parse_raw_data_item _ _);
-    let vpl = vpattern_replace_erased (fun vpl -> A.pts_to payload _ vpl `star` (A.pts_to payload _ vpl `implies_` LPS.aparse CborST.parse_raw_data_item cs.cbor_serialized_payload va')) in
-    let vperm = vpattern_replace (fun vperm -> A.pts_to payload vperm _ `star` (A.pts_to payload vperm _ `implies_` LPS.aparse CborST.parse_raw_data_item cs.cbor_serialized_payload va')) in
+      (raw_data_item_match _ _ _);
+    [@@inline_let]
     let c' : cbor_string = {
       cbor_string_type = typ;
       cbor_string_length = len;
       cbor_string_payload = payload;
-      permission = vperm;
     }
     in
-    noop ();
-    intro_implies
-      (raw_data_item_match_string0 (CBOR_Case_String c') (Ghost.reveal va))
-      (raw_data_item_match_serialized0 c (Ghost.reveal va))
-      (A.pts_to payload vperm vpl `implies_` LPS.aparse CborST.parse_raw_data_item cs.cbor_serialized_payload va')
-      (fun _ ->
-        let _ = gen_elim () in
-        rewrite (A.pts_to _ _ _) (A.pts_to payload vperm vpl);
-        elim_implies
-          (A.pts_to payload vperm vpl)
-          (LPS.aparse CborST.parse_raw_data_item cs.cbor_serialized_payload va');
-        noop ()
-      );
-    rewrite_with_implies
-      (raw_data_item_match_string0 (CBOR_Case_String c') (Ghost.reveal va))
-      (raw_data_item_match (CBOR_Case_String c') (Ghost.reveal va));
+    vpattern_rewrite_with_implies
+      (fun a -> A.pts_to a _ _)
+      c'.cbor_string_payload;
     implies_trans
-      (raw_data_item_match (CBOR_Case_String c') (Ghost.reveal va))
-      (raw_data_item_match_string0 (CBOR_Case_String c') (Ghost.reveal va))
-      (raw_data_item_match_serialized0 c (Ghost.reveal va));
-    implies_trans
-      (raw_data_item_match (CBOR_Case_String c') (Ghost.reveal va))
-      (raw_data_item_match_serialized0 c (Ghost.reveal va))
-      (raw_data_item_match c (Ghost.reveal va));
+      (A.pts_to _ _ _)
+      (A.pts_to _ _ _)
+      (raw_data_item_match _ _ _);
     return c'
-
-let destr_cbor_string
-  (#va: Ghost.erased Cbor.raw_data_item)
-  (c: cbor {Cbor.String? va})
-: STT cbor_string
-    (raw_data_item_match c (Ghost.reveal va))
-    (fun c' -> exists_ (fun vc' ->
-      A.pts_to c'.cbor_string_payload c'.permission vc' `star`
-      (A.pts_to c'.cbor_string_payload c'.permission vc' `implies_` raw_data_item_match c (Ghost.reveal va)) `star`
-      pure (
-        U64.v c'.cbor_string_length == Seq.length vc' /\
-        c'.cbor_string_type == Cbor.String?.typ va /\
-        vc' == Cbor.String?.v va
-    )))
-= let c' = destr_cbor_string' c in
-  rewrite_with_implies
-    (raw_data_item_match (CBOR_Case_String c') (Ghost.reveal va))
-    (raw_data_item_match_string0 (CBOR_Case_String c') (Ghost.reveal va));
-  let _ = gen_elim () in
-  vpattern_rewrite (fun a -> A.pts_to a _ _) c'.cbor_string_payload;
-  vpattern_rewrite (fun p -> A.pts_to _ p _) c'.permission;
-  let vc' = vpattern_replace_erased (A.pts_to _ _) in
-  intro_implies
-    (A.pts_to c'.cbor_string_payload c'.permission vc')
-    (raw_data_item_match_string0 (CBOR_Case_String c') (Ghost.reveal va))
-    (pure (raw_data_item_match_string_prop (CBOR_Case_String c') (Ghost.reveal va) c'.cbor_string_payload c'.permission vc')) // FIXME: WHY WHY WHY?
-    (fun _ ->
-      noop ()
-    );
-  implies_trans
-    (A.pts_to c'.cbor_string_payload c'.permission vc')
-    (raw_data_item_match_string0 (CBOR_Case_String c') (Ghost.reveal va))
-    (raw_data_item_match (CBOR_Case_String c') (Ghost.reveal va));
-  implies_trans
-    (A.pts_to c'.cbor_string_payload c'.permission vc')
-    (raw_data_item_match (CBOR_Case_String c') (Ghost.reveal va))
-    (raw_data_item_match c (Ghost.reveal va));
-  intro_exists (Ghost.reveal vc') (fun vc' -> // FIXME: WHY WHY WHY?
-    A.pts_to c'.cbor_string_payload c'.permission vc' `star`
-      (A.pts_to c'.cbor_string_payload c'.permission vc' `implies_` raw_data_item_match c (Ghost.reveal va)) `star`
-      pure (
-        U64.v c'.cbor_string_length == Seq.length vc' /\
-        c'.cbor_string_type == Cbor.String?.typ va /\
-        vc' == Cbor.String?.v va
-    )  
-  );
-  return c'
 
 #push-options "--z3rlimit 64"
 #restart-solver
@@ -906,7 +1067,7 @@ let size_comp_for_string
   (va: Ghost.erased Cbor.raw_data_item)
   (c: cbor { Cbor.String? va })
 : Tot (cbor_size_comp_for va c)
-= fun sz perr ->
+= fun #p sz perr ->
     let _ = A.intro_fits_u64 () in
     let c' = destr_cbor_string c in
     let _ = gen_elim () in
@@ -914,7 +1075,7 @@ let size_comp_for_string
     let _ = gen_elim () in
     elim_implies
       (A.pts_to _ _ _)
-      (raw_data_item_match _ _);
+      (raw_data_item_match p _ _);
     return res
 
 let serialize_cbor_string_eq
@@ -939,7 +1100,7 @@ let l2r_write_cbor_string
   (va: Ghost.erased Cbor.raw_data_item)
   (c: cbor {Cbor.String? va})
 : Tot (cbor_l2r_writer_for va c)
-= fun #vout out ->
+= fun #p #vout out ->
   let _ = A.intro_fits_u64 () in
   serialize_cbor_string_eq va;
   noop ();
@@ -967,123 +1128,120 @@ let l2r_write_cbor_string
   let vres = LPS.intro_aparse_with_serializer CborST.serialize_raw_data_item va res in
   elim_implies
     (A.pts_to _ _ _)
-    (raw_data_item_match c (Ghost.reveal va));
-  assert_ (cbor_l2r_writer_for_post va c vout out res vres vout'); // FIXME: WHY WHY WHY?
+    (raw_data_item_match p c (Ghost.reveal va));
+  assert_ (cbor_l2r_writer_for_post p va c vout out res vres vout'); // FIXME: WHY WHY WHY?
   return res
 
 #pop-options
 
 let constr_cbor_string
   #va #p typ a len
-= [@@inline_let]
-  let c' = CBOR_Case_String ({
-    cbor_string_type = typ;
-    cbor_string_payload = a;
-    cbor_string_length = len;
-    permission = p;
-  })
+= let fp = GR.alloc () in
+  [@@inline_let]
+  let c' = CBOR_Case_String
+    ({
+      cbor_string_type = typ;
+      cbor_string_payload = a;
+      cbor_string_length = len;
+    })
+    fp
+    p
   in
   noop ();
   rewrite_with_implies
-    (raw_data_item_match_string0 c' (Cbor.String typ va))
-    (raw_data_item_match c' (Cbor.String typ va));
+    (raw_data_item_match_string0 full_perm c' (Cbor.String typ va))
+    (raw_data_item_match full_perm c' (Cbor.String typ va));
   intro_implies
-    (raw_data_item_match_string0 c' (Cbor.String typ va))
+    (raw_data_item_match_string0 full_perm c' (Cbor.String typ va))
     (A.pts_to a p va)
     emp
     (fun _ ->
       let _ = gen_elim () in
+      GR.free _;
       rewrite (A.pts_to _ _ _) (A.pts_to a p va)
     );
   implies_trans
-    (raw_data_item_match c' (Cbor.String typ (va)))
-    (raw_data_item_match_string0 c' (Cbor.String typ (va)))
+    (raw_data_item_match full_perm c' (Cbor.String typ (va)))
+    (raw_data_item_match_string0 full_perm c' (Cbor.String typ (va)))
     (A.pts_to a p va);
   return c'
 
 let raw_data_item_match_array_intro
   (#opened: _)
+  (#p: perm)
   (#c': Seq.seq cbor)
   (#v': list Cbor.raw_data_item)
+  (fp: cbor_footprint_t)
   (a: A.array cbor)
   (len: U64.t {
     U64.v len == List.Tot.length v'
   })
 : STGhostT unit opened
-    (A.pts_to a full_perm c' `star`
-      raw_data_item_array_match c' v')
+    (A.pts_to a p c' `star`
+      GR.pts_to fp p () `star`
+      raw_data_item_array_match p c' v')
     (fun _ ->
       raw_data_item_match
-        (CBOR_Case_Array ({
-          cbor_array_length = len;
-          cbor_array_payload = a;
-          footprint = c';
-        }))
+        p
+        (CBOR_Case_Array
+          ({
+            cbor_array_length = len;
+            cbor_array_payload = a;
+            footprint = c';
+          })
+          fp
+        )
         (Cbor.Array v')
     )
 = noop ();
   rewrite_with_tactic
     (raw_data_item_match_array0
-      (CBOR_Case_Array ({
-        cbor_array_length = len;
-        cbor_array_payload = a;
-        footprint = c';
-      }))
+      p
+      (CBOR_Case_Array
+        ({
+          cbor_array_length = len;
+          cbor_array_payload = a;
+          footprint = c';
+        })
+        fp
+      )
       (Cbor.Array v')
-      raw_data_item_array_match
+      (raw_data_item_array_match p)
     )
-    (raw_data_item_match _ _)
+    (raw_data_item_match p _ _)
 
 let raw_data_item_match_array_elim
   (#opened: _)
+  (#p: perm)
   (a: cbor_array)
+  (fp: cbor_footprint_t)
   (v: Cbor.raw_data_item)
 : STGhost (squash (Cbor.Array? v)) opened
-    (raw_data_item_match (CBOR_Case_Array a) v)
+    (raw_data_item_match p (CBOR_Case_Array a fp) v)
     (fun _ ->
-      A.pts_to a.cbor_array_payload full_perm a.footprint `star`
-      raw_data_item_array_match a.footprint (Cbor.Array?.v v)
+      A.pts_to a.cbor_array_payload p a.footprint `star`
+      GR.pts_to fp p () `star`
+      raw_data_item_array_match p a.footprint (Cbor.Array?.v v)
     )
     True
     (fun _ -> U64.v a.cbor_array_length == List.Tot.length (Cbor.Array?.v v))
 = raw_data_item_match_get_case _;
   let sq : squash (Cbor.Array? v) = () in
   let Cbor.Array v' = v in
-  vpattern_rewrite (raw_data_item_match _) (Cbor.Array v');
+  vpattern_rewrite (raw_data_item_match p _) (Cbor.Array v');
   rewrite_with_tactic
-    (raw_data_item_match _ _)
-    (raw_data_item_match_array0 (CBOR_Case_Array a) (Cbor.Array v') raw_data_item_array_match);
+    (raw_data_item_match p _ _)
+    (raw_data_item_match_array0 p (CBOR_Case_Array a fp) (Cbor.Array v') (raw_data_item_array_match p));
   let _ = gen_elim () in
-  rewrite (A.pts_to _ _ _) (A.pts_to a.cbor_array_payload full_perm a.footprint);
-  rewrite (raw_data_item_array_match _ _) (raw_data_item_array_match a.footprint (Cbor.Array?.v v));
+  rewrite (A.pts_to _ _ _) (A.pts_to a.cbor_array_payload p a.footprint);
+  rewrite (GR.pts_to _ _ _) (GR.pts_to fp p ());
+  rewrite (raw_data_item_array_match p _ _) (raw_data_item_array_match p a.footprint (Cbor.Array?.v v));
   sq
 
 let constr_cbor_array
-  (#c': Ghost.erased (Seq.seq cbor))
-  (#v': Ghost.erased (list Cbor.raw_data_item))
-  (a: A.array cbor)
-  (len: U64.t {
-    U64.v len == List.Tot.length v'
-  })
-: ST cbor
-    (A.pts_to a full_perm c' `star`
-      raw_data_item_array_match c' v')
-    (fun res ->
-      raw_data_item_match res (Cbor.Array v') `star`
-      (raw_data_item_match res (Cbor.Array v') `implies_`
-        (A.pts_to a full_perm c' `star`
-          raw_data_item_array_match c' v')
-      )
-    )
-    True
-    (fun res ->
-      res == CBOR_Case_Array ({
-        cbor_array_payload = a;
-        cbor_array_length = len;
-        footprint = c';
-      })
-    )
-= [@@inline_let]
+  #c' #v' a len
+= let fp = GR.alloc () in
+  [@@inline_let]
   let ares : cbor_array = {
     cbor_array_length = len;
     cbor_array_payload = a;
@@ -1091,52 +1249,70 @@ let constr_cbor_array
   }
   in
   [@@inline_let]
-  let res = CBOR_Case_Array ares in
-  raw_data_item_match_array_intro a len;
-  rewrite (raw_data_item_match _ _) (raw_data_item_match res (Cbor.Array v'));
+  let res = CBOR_Case_Array ares fp in
+  raw_data_item_match_array_intro fp a len;
+  rewrite (raw_data_item_match full_perm _ _) (raw_data_item_match full_perm res (Cbor.Array v'));
   intro_implies
-    (raw_data_item_match res (Cbor.Array v'))
+    (raw_data_item_match full_perm res (Cbor.Array v'))
     (A.pts_to a full_perm c' `star`
-      raw_data_item_array_match c' v'
+      raw_data_item_array_match full_perm c' v'
     )
     emp
     (fun _ ->
-      rewrite (raw_data_item_match _ _) (raw_data_item_match (CBOR_Case_Array ares) (Cbor.Array v'));
-      let _ = raw_data_item_match_array_elim _ _ in
+      rewrite (raw_data_item_match full_perm _ _) (raw_data_item_match full_perm (CBOR_Case_Array ares fp) (Cbor.Array v'));
+      let _ = raw_data_item_match_array_elim _ _ _ in
       rewrite (A.pts_to _ _ _) (A.pts_to a full_perm c');
-      rewrite (raw_data_item_array_match _ _) (raw_data_item_array_match c' v')
+      GR.free _;
+      rewrite (raw_data_item_array_match full_perm _ _) (raw_data_item_array_match full_perm c' v')
     );
   return res
 
 let destr_cbor_array
-  #v a
+  (#p: perm)
+  (#v: Ghost.erased Cbor.raw_data_item)
+  (a: cbor)
+: ST cbor_array
+    (raw_data_item_match p a v)
+    (fun res ->
+      A.pts_to res.cbor_array_payload p res.footprint `star`
+      raw_data_item_array_match p res.footprint (maybe_cbor_array v) `star`
+      ((A.pts_to res.cbor_array_payload p res.footprint `star`
+        raw_data_item_array_match p res.footprint (maybe_cbor_array v)) `implies_`
+        raw_data_item_match p a v
+      )
+    )
+    (CBOR_Case_Array? a)
+    (fun res ->
+      Cbor.Array? v /\
+      U64.v res.cbor_array_length == List.Tot.length (maybe_cbor_array v)
+    )
 = raw_data_item_match_get_case _;
-  let CBOR_Case_Array res = a in
+  let CBOR_Case_Array res fp = a in
   vpattern_rewrite
-    (fun a -> raw_data_item_match a _)
-    (CBOR_Case_Array res);
-  let _ = raw_data_item_match_array_elim _ _ in
-  vpattern_rewrite (raw_data_item_array_match _) (maybe_cbor_array v);
+    (fun a -> raw_data_item_match p a _)
+    (CBOR_Case_Array res fp);
+  let _ = raw_data_item_match_array_elim _ _ _ in
+  vpattern_rewrite (raw_data_item_array_match p _) (maybe_cbor_array v);
   intro_implies
-    (A.pts_to res.cbor_array_payload full_perm res.footprint `star`
-      raw_data_item_array_match res.footprint (maybe_cbor_array v))
-    (raw_data_item_match a v)
-    emp
+    (A.pts_to res.cbor_array_payload p res.footprint `star`
+      raw_data_item_array_match p res.footprint (maybe_cbor_array v))
+    (raw_data_item_match p a v)
+    (GR.pts_to _ _ _)
     (fun _ ->
-      raw_data_item_match_array_intro _ res.cbor_array_length;
-      rewrite (raw_data_item_match _ _) (raw_data_item_match _ _)
+      raw_data_item_match_array_intro fp _ res.cbor_array_length;
+      rewrite (raw_data_item_match p _ _) (raw_data_item_match p _ _)
     );
   return res
 
 let cbor_array_length
-  #v a
+  #p #v a
 = raw_data_item_match_get_case a;
   match a with
-  | CBOR_Case_Array _ ->
+  | CBOR_Case_Array _ _ ->
     let a' = destr_cbor_array a in
     elim_implies
-      (A.pts_to _ _ _ `star` raw_data_item_array_match _ _)
-      (raw_data_item_match _ _);
+      (A.pts_to _ _ _ `star` raw_data_item_array_match p _ _)
+      (raw_data_item_match p _ _);
     return a'.cbor_array_length
   | _ ->
     let s = destr_cbor_serialized a in
@@ -1144,10 +1320,11 @@ let cbor_array_length
     let res = CborST.read_argument_as_uint64 s.cbor_serialized_payload in
     elim_implies
       (LPS.aparse CborST.parse_raw_data_item _ _)
-      (raw_data_item_match _ _);
+      (raw_data_item_match p _ _);
     return res
 
 let cbor_array_index_case_array
+  (#p: perm)
   (#v: Ghost.erased Cbor.raw_data_item)
   (a: cbor)
   (i: SZ.t {
@@ -1156,51 +1333,52 @@ let cbor_array_index_case_array
     CBOR_Case_Array? a
   })
 : STT cbor
-    (raw_data_item_match a v)
+    (raw_data_item_match p a v)
     (fun a' ->
-      raw_data_item_match a' (List.Tot.index (Cbor.Array?.v v) (SZ.v i)) `star`
-      (raw_data_item_match a' (List.Tot.index (Cbor.Array?.v v) (SZ.v i)) `implies_`
-        raw_data_item_match a v)
+      raw_data_item_match p a' (List.Tot.index (Cbor.Array?.v v) (SZ.v i)) `star`
+      (raw_data_item_match p a' (List.Tot.index (Cbor.Array?.v v) (SZ.v i)) `implies_`
+        raw_data_item_match p a v)
     )
 = raw_data_item_match_get_case a;
   noop ();
   let ar = destr_cbor_array a in
   A.pts_to_length ar.cbor_array_payload _;
-  SM.seq_list_match_length raw_data_item_match ar.footprint (maybe_cbor_array v);
+  SM.seq_list_match_length (raw_data_item_match p) ar.footprint (maybe_cbor_array v);
   let res = A.index ar.cbor_array_payload i in
   intro_implies
-    (raw_data_item_array_match ar.footprint (maybe_cbor_array v))
-    (raw_data_item_match a v)
+    (raw_data_item_array_match p ar.footprint (maybe_cbor_array v))
+    (raw_data_item_match p a v)
     (A.pts_to _ _ _ `star`
-      ((A.pts_to _ _ _ `star` raw_data_item_array_match _ _) `implies_` raw_data_item_match _ _)
+      ((A.pts_to _ _ _ `star` raw_data_item_array_match p _ _) `implies_` raw_data_item_match p _ _)
     )
     (fun _ ->
        elim_implies
-       (A.pts_to _ _ _ `star` raw_data_item_array_match _ _)
-       (raw_data_item_match _ _)
+       (A.pts_to _ _ _ `star` raw_data_item_array_match p _ _)
+       (raw_data_item_match p _ _)
     );
   rewrite_with_implies
-    (raw_data_item_array_match ar.footprint (maybe_cbor_array v))
-    (SM.seq_list_match ar.footprint (maybe_cbor_array v) raw_data_item_match);
+    (raw_data_item_array_match p ar.footprint (maybe_cbor_array v))
+    (SM.seq_list_match ar.footprint (maybe_cbor_array v) (raw_data_item_match p));
   implies_trans
-    (SM.seq_list_match ar.footprint (maybe_cbor_array v) raw_data_item_match)
-    (raw_data_item_array_match ar.footprint (maybe_cbor_array v))
-    (raw_data_item_match a v);
-  let _ = SM.seq_list_match_index raw_data_item_match ar.footprint (maybe_cbor_array v) (SZ.v i) in
+    (SM.seq_list_match ar.footprint (maybe_cbor_array v) (raw_data_item_match p))
+    (raw_data_item_array_match p ar.footprint (maybe_cbor_array v))
+    (raw_data_item_match p a v);
+  let _ = SM.seq_list_match_index (raw_data_item_match p) ar.footprint (maybe_cbor_array v) (SZ.v i) in
   implies_trans
-    (raw_data_item_match (Seq.index ar.footprint (SZ.v i)) (List.Tot.index (maybe_cbor_array v) (SZ.v i)))
-    (SM.seq_list_match ar.footprint (maybe_cbor_array v) raw_data_item_match)
-    (raw_data_item_match a v);
+    (raw_data_item_match p (Seq.index ar.footprint (SZ.v i)) (List.Tot.index (maybe_cbor_array v) (SZ.v i)))
+    (SM.seq_list_match ar.footprint (maybe_cbor_array v) (raw_data_item_match p))
+    (raw_data_item_match p a v);
   rewrite_with_implies
-    (raw_data_item_match (Seq.index ar.footprint (SZ.v i)) (List.Tot.index (maybe_cbor_array v) (SZ.v i)))
-    (raw_data_item_match res (List.Tot.index (Cbor.Array?.v v) (SZ.v i)));
+    (raw_data_item_match p (Seq.index ar.footprint (SZ.v i)) (List.Tot.index (maybe_cbor_array v) (SZ.v i)))
+    (raw_data_item_match p res (List.Tot.index (Cbor.Array?.v v) (SZ.v i)));
   implies_trans
-    (raw_data_item_match res (List.Tot.index (Cbor.Array?.v v) (SZ.v i)))
-    (raw_data_item_match (Seq.index ar.footprint (SZ.v i)) (List.Tot.index (maybe_cbor_array v) (SZ.v i)))
-    (raw_data_item_match a v);
+    (raw_data_item_match p res (List.Tot.index (Cbor.Array?.v v) (SZ.v i)))
+    (raw_data_item_match p (Seq.index ar.footprint (SZ.v i)) (List.Tot.index (maybe_cbor_array v) (SZ.v i)))
+    (raw_data_item_match p a v);
   return res
 
 let cbor_array_index_case_serialized
+  (#p: perm)
   (#v: Ghost.erased Cbor.raw_data_item)
   (a: cbor)
   (i: SZ.t {
@@ -1209,13 +1387,14 @@ let cbor_array_index_case_serialized
     CBOR_Case_Serialized? a
   })
 : STT cbor
-    (raw_data_item_match a v)
+    (raw_data_item_match p a v)
     (fun a' ->
-      raw_data_item_match a' (List.Tot.index (Cbor.Array?.v v) (SZ.v i)) `star`
-      (raw_data_item_match a' (List.Tot.index (Cbor.Array?.v v) (SZ.v i)) `implies_`
-        raw_data_item_match a v)
+      raw_data_item_match p a' (List.Tot.index (Cbor.Array?.v v) (SZ.v i)) `star`
+      (raw_data_item_match p a' (List.Tot.index (Cbor.Array?.v v) (SZ.v i)) `implies_`
+        raw_data_item_match p a v)
     )
-= let s = destr_cbor_serialized a in
+= raw_data_item_match_perm_le_full_perm a;
+  let s = destr_cbor_serialized a in
   let _ = gen_elim () in
   let n = Ghost.hide (List.Tot.length (Cbor.Array?.v v)) in
   let a = CBOR.SteelST.Raw.Array.focus_array_with_ghost_length n s.cbor_serialized_payload in
@@ -1223,38 +1402,38 @@ let cbor_array_index_case_serialized
   implies_trans
     (LPS.aparse (LPS.parse_nlist n CborST.parse_raw_data_item) _ _)
     (LPS.aparse CborST.parse_raw_data_item _ _)
-    (raw_data_item_match _ _);
+    (raw_data_item_match p _ _);
   let _ = LPS.aparse_nlist_aparse_list_with_implies CborST.parse_raw_data_item n a in
   implies_trans
     (LPS.aparse (LPS.parse_list CborST.parse_raw_data_item) _ _)
     (LPS.aparse (LPS.parse_nlist n CborST.parse_raw_data_item) _ _)
-    (raw_data_item_match _ _);
+    (raw_data_item_match p _ _);
   let elt = LowParse.SteelST.List.Nth.list_nth_with_implies CborST.jump_raw_data_item a i in
   let _ = gen_elim () in
   implies_trans
     (LPS.aparse CborST.parse_raw_data_item _ _)
     (LPS.aparse (LPS.parse_list CborST.parse_raw_data_item) _ _)
-    (raw_data_item_match _ _);
+    (raw_data_item_match p _ _);
   let sz = LPS.get_parsed_size CborST.jump_raw_data_item elt in
-  let res = read_valid_cbor_from_buffer_with_size_strong elt sz in
+  let res = read_valid_cbor_from_buffer_with_size_strong p elt sz in
   implies_trans
-    (raw_data_item_match res _)
+    (raw_data_item_match p res _)
     (LPS.aparse CborST.parse_raw_data_item _ _)
-    (raw_data_item_match _ _);
+    (raw_data_item_match p _ _);
   vpattern_rewrite_with_implies
-    (raw_data_item_match res)
+    (raw_data_item_match p res)
     (List.Tot.index (Cbor.Array?.v v) (SZ.v i));
   implies_trans
-    (raw_data_item_match res _)
-    (raw_data_item_match res _)
-    (raw_data_item_match _ _);
+    (raw_data_item_match p res _)
+    (raw_data_item_match p res _)
+    (raw_data_item_match p _ _);
   return res
     
 let cbor_array_index
   a i
 = raw_data_item_match_get_case a;
   match a with
-  | CBOR_Case_Array _ ->
+  | CBOR_Case_Array _ _ ->
     return (cbor_array_index_case_array a i)
   | _ ->
     return (cbor_array_index_case_serialized a i)
@@ -1263,22 +1442,26 @@ let cbor_array_index
 let dummy_cbor_array_iterator = {
   cbor_array_iterator_length = 0uL;
   cbor_array_iterator_payload = CBOR_Array_Iterator_Payload_Array A.null Seq.empty;
+  footprint = magic ();
 }
 
 [@@__reduce__]
 let cbor_array_iterator_match_array
+  (p: perm)
   (c: cbor_array_iterator_t)
   (l: list Cbor.raw_data_item)
 : Tot vprop
 = exists_ (fun a -> exists_ (fun fp ->
-    A.pts_to a full_perm fp `star`
-    raw_data_item_array_match fp l `star`
+    GR.pts_to c.footprint p () `star`
+    A.pts_to a p fp `star`
+    raw_data_item_array_match p fp l `star`
     pure (
       U64.v c.cbor_array_iterator_length == List.Tot.length l /\
       c.cbor_array_iterator_payload == CBOR_Array_Iterator_Payload_Array a (Ghost.hide fp)
   )))
 
 let cbor_array_iterator_match_serialized_prop
+  (p: perm)
   (c: cbor_array_iterator_t)
   (l: list Cbor.raw_data_item)
   (a: LPS.byte_array)
@@ -1286,118 +1469,136 @@ let cbor_array_iterator_match_serialized_prop
 : Tot prop
 = 
   fp.LPS.contents == l /\
-  c.cbor_array_iterator_payload == CBOR_Array_Iterator_Payload_Serialized a (LPS.array_of fp)
+  begin match c.cbor_array_iterator_payload with
+  | CBOR_Array_Iterator_Payload_Serialized a' fp' ->
+    a == a' /\
+    LPS.array_of fp == LPA.set_array_perm fp' (p `prod_perm` LPA.array_perm fp')
+  | _ -> False
+  end
 
 [@@__reduce__]
 let cbor_array_iterator_match_serialized
+  (p: perm)
   (c: cbor_array_iterator_t)
   (l: list Cbor.raw_data_item)
 : Tot vprop
 = exists_ (fun a -> exists_ (fun fp ->
+    GR.pts_to c.footprint p () `star`
     LPS.aparse (LPS.parse_nlist (U64.v c.cbor_array_iterator_length) CborST.parse_raw_data_item) a fp `star`
-    pure (cbor_array_iterator_match_serialized_prop c l a fp)
+    pure (cbor_array_iterator_match_serialized_prop p c l a fp)
   ))
 
 let cbor_array_iterator_match
-  c l
+  p c l
 = match c.cbor_array_iterator_payload with
-  | CBOR_Array_Iterator_Payload_Array _ _ -> cbor_array_iterator_match_array c l
-  | _ -> cbor_array_iterator_match_serialized c l
+  | CBOR_Array_Iterator_Payload_Array _ _ -> cbor_array_iterator_match_array p c l
+  | _ -> cbor_array_iterator_match_serialized p c l
 
-#push-options "--z3rlimit 16"
+#push-options "--z3rlimit 32"
 #restart-solver
 
 let cbor_array_iterator_match_length
   (#opened: _)
+  (#p: perm)
   (#l: Ghost.erased (list Cbor.raw_data_item))
   (i: cbor_array_iterator_t)
 : STGhost unit opened
-    (cbor_array_iterator_match i l)
-    (fun _ -> cbor_array_iterator_match i l)
+    (cbor_array_iterator_match p i l)
+    (fun _ -> cbor_array_iterator_match p i l)
     True
     (fun _ -> U64.v i.cbor_array_iterator_length == List.Tot.length l)
 = match i.cbor_array_iterator_payload with
   | CBOR_Array_Iterator_Payload_Array _ _ ->
     rewrite
-      (cbor_array_iterator_match i l)
-      (cbor_array_iterator_match_array i l);
+      (cbor_array_iterator_match p i l)
+      (cbor_array_iterator_match_array p i l);
     let _ = gen_elim () in
     rewrite
-      (cbor_array_iterator_match_array i l)
-      (cbor_array_iterator_match i l)
+      (cbor_array_iterator_match_array p i l)
+      (cbor_array_iterator_match p i l)
   | CBOR_Array_Iterator_Payload_Serialized _ _ ->
     rewrite
-      (cbor_array_iterator_match i l)
-      (cbor_array_iterator_match_serialized i l);
+      (cbor_array_iterator_match p i l)
+      (cbor_array_iterator_match_serialized p i l);
     let _ = gen_elim () in
     rewrite
-      (cbor_array_iterator_match_serialized i l)
-      (cbor_array_iterator_match i l)
+      (cbor_array_iterator_match_serialized p i l)
+      (cbor_array_iterator_match p i l)
 
 #pop-options
 
 let cbor_array_iterator_init_array
+  (#p: perm)
   (#v: Ghost.erased Cbor.raw_data_item)
   (a: cbor { Cbor.Array? v /\ CBOR_Case_Array? a })
 : STT cbor_array_iterator_t
-    (raw_data_item_match a v)
+    (raw_data_item_match p a v)
     (fun i ->
-      cbor_array_iterator_match i (Cbor.Array?.v v) `star`
-      (cbor_array_iterator_match i (Cbor.Array?.v v) `implies_`
-        raw_data_item_match a v)
+      cbor_array_iterator_match p i (Cbor.Array?.v v) `star`
+      (cbor_array_iterator_match p i (Cbor.Array?.v v) `implies_`
+        raw_data_item_match p a v)
     )
-= let len = cbor_array_length a in
+= raw_data_item_match_perm_le_full_perm a;
+  let len = cbor_array_length a in
   let ar = destr_cbor_array a in
+  let fp = GR.alloc () in // I could reuse the footprint from `a`, but `destr_cbor_array` does not expose it
+  gref_lower_perm fp p;
   let res = {
     cbor_array_iterator_length = len;
     cbor_array_iterator_payload = CBOR_Array_Iterator_Payload_Array ar.cbor_array_payload ar.footprint;
+    footprint = fp;
   }
   in
-  noop ();
+  vpattern_rewrite_with_implies (fun r -> GR.pts_to r _ _) res.footprint;
+  implies_trans (GR.pts_to res.footprint p ()) (GR.pts_to fp p ()) (GR.pts_to fp full_perm ());
   rewrite_with_implies
-    (cbor_array_iterator_match_array res (maybe_cbor_array v))
-    (cbor_array_iterator_match res (Cbor.Array?.v v));
+    (cbor_array_iterator_match_array p res (maybe_cbor_array v))
+    (cbor_array_iterator_match p res (Cbor.Array?.v v));
   intro_implies
-    (cbor_array_iterator_match_array res (maybe_cbor_array v))
-    (A.pts_to ar.cbor_array_payload full_perm ar.footprint `star`
-      raw_data_item_array_match ar.footprint (maybe_cbor_array v)
+    (cbor_array_iterator_match_array p res (maybe_cbor_array v))
+    (A.pts_to ar.cbor_array_payload p ar.footprint `star`
+      raw_data_item_array_match p ar.footprint (maybe_cbor_array v)
     )
-    emp
+    (GR.pts_to res.footprint p () `implies_` GR.pts_to fp full_perm ())
     (fun _ ->
       let _ = gen_elim () in
+      elim_implies (GR.pts_to _ _ _) (GR.pts_to _ _ _);
+      GR.free _;
       rewrite
         (A.pts_to _ _ _)
-        (A.pts_to ar.cbor_array_payload full_perm ar.footprint);
+        (A.pts_to ar.cbor_array_payload p ar.footprint);
       rewrite
-        (raw_data_item_array_match _ _)
-        (raw_data_item_array_match ar.footprint (maybe_cbor_array v))
+        (raw_data_item_array_match p _ _)
+        (raw_data_item_array_match p ar.footprint (maybe_cbor_array v))
     );
   implies_trans
-    (cbor_array_iterator_match_array res (maybe_cbor_array v))
-    (A.pts_to ar.cbor_array_payload full_perm ar.footprint `star`
-      raw_data_item_array_match ar.footprint (maybe_cbor_array v)
+    (cbor_array_iterator_match_array p res (maybe_cbor_array v))
+    (A.pts_to ar.cbor_array_payload p ar.footprint `star`
+      raw_data_item_array_match p ar.footprint (maybe_cbor_array v)
     )
-    (raw_data_item_match a v);
+    (raw_data_item_match p a v);
   implies_trans
-    (cbor_array_iterator_match res (Cbor.Array?.v v))
-    (cbor_array_iterator_match_array res (maybe_cbor_array v))
-    (raw_data_item_match a v);
+    (cbor_array_iterator_match p res (Cbor.Array?.v v))
+    (cbor_array_iterator_match_array p res (maybe_cbor_array v))
+    (raw_data_item_match p a v);
   return res
 
 #push-options "--z3rlimit 64"
 #restart-solver
 
 let cbor_array_iterator_init_serialized
+  (#p: perm)
   (#v: Ghost.erased Cbor.raw_data_item)
   (a: cbor { Cbor.Array? v /\ CBOR_Case_Serialized? a })
 : STT cbor_array_iterator_t
-    (raw_data_item_match a v)
+    (raw_data_item_match p a v)
     (fun i ->
-      cbor_array_iterator_match i (Cbor.Array?.v v) `star`
-      (cbor_array_iterator_match i (Cbor.Array?.v v) `implies_`
-        raw_data_item_match a v)
+      cbor_array_iterator_match p i (Cbor.Array?.v v) `star`
+      (cbor_array_iterator_match p i (Cbor.Array?.v v) `implies_`
+        raw_data_item_match p a v)
     )
-= let len = cbor_array_length a in
+= raw_data_item_match_perm_le_full_perm a;
+  let len = cbor_array_length a in
   let s = destr_cbor_serialized a in
   let _ = gen_elim () in
   let ar = CBOR.SteelST.Raw.Array.focus_array_with_ghost_length (U64.v len) s.cbor_serialized_payload in
@@ -1405,40 +1606,47 @@ let cbor_array_iterator_init_serialized
   implies_trans
     (LPS.aparse (LPS.parse_nlist (U64.v len) CborST.parse_raw_data_item) _ _)
     (LPS.aparse CborST.parse_raw_data_item _ _)
-    (raw_data_item_match a v);
+    (raw_data_item_match p a v);
   let var0 = vpattern (LPS.aparse (LPS.parse_nlist (U64.v len) CborST.parse_raw_data_item) _) in
+  let fp = GR.alloc () in // same as above, I could use the footprint from `a` but `destr_cbor_serialized` does not expose it
+  gref_lower_perm fp p;
   [@@inline_let]
   let res = {
     cbor_array_iterator_length = len;
-    cbor_array_iterator_payload = CBOR_Array_Iterator_Payload_Serialized ar (LPS.array_of var0);
+    cbor_array_iterator_payload = CBOR_Array_Iterator_Payload_Serialized ar (LPA.set_array_perm (LPS.array_of var0) (LPA.array_perm (LPS.array_of var0) `div_perm` p));
+    footprint = fp;
   }
   in
+  vpattern_rewrite_with_implies (fun r -> GR.pts_to r _ _) res.footprint;
+  implies_trans (GR.pts_to res.footprint p ()) (GR.pts_to fp p ()) (GR.pts_to fp full_perm ());
   let var = LPS.rewrite_aparse_with_implies ar (LPS.parse_nlist (U64.v res.cbor_array_iterator_length) CborST.parse_raw_data_item) in
   implies_trans
     (LPS.aparse (LPS.parse_nlist (U64.v res.cbor_array_iterator_length) CborST.parse_raw_data_item) ar var)
     (LPS.aparse (LPS.parse_nlist (U64.v len) CborST.parse_raw_data_item) _ _)
-    (raw_data_item_match a v);
+    (raw_data_item_match p a v);
   rewrite_with_implies
-    (cbor_array_iterator_match_serialized res (Cbor.Array?.v v))
-    (cbor_array_iterator_match res (Cbor.Array?.v v));
+    (cbor_array_iterator_match_serialized p res (Cbor.Array?.v v))
+    (cbor_array_iterator_match p res (Cbor.Array?.v v));
   intro_implies
-    (cbor_array_iterator_match_serialized res (Cbor.Array?.v v))
+    (cbor_array_iterator_match_serialized p res (Cbor.Array?.v v))
     (LPS.aparse (LPS.parse_nlist (U64.v res.cbor_array_iterator_length) CborST.parse_raw_data_item) ar var)
-    emp
+    (GR.pts_to res.footprint p () `implies_` GR.pts_to fp full_perm ())
     (fun _ ->
       let _ = gen_elim () in
+      elim_implies (GR.pts_to _ _ _) (GR.pts_to _ _ _);
+      GR.free _;
       rewrite
         (LPS.aparse (LPS.parse_nlist (U64.v res.cbor_array_iterator_length) CborST.parse_raw_data_item) _ _)
         (LPS.aparse (LPS.parse_nlist (U64.v res.cbor_array_iterator_length) CborST.parse_raw_data_item) ar var)
     );
   implies_trans
-    (cbor_array_iterator_match res (Cbor.Array?.v v))
-    (cbor_array_iterator_match_serialized res (Cbor.Array?.v v))
+    (cbor_array_iterator_match p res (Cbor.Array?.v v))
+    (cbor_array_iterator_match_serialized p res (Cbor.Array?.v v))
     (LPS.aparse (LPS.parse_nlist (U64.v res.cbor_array_iterator_length) CborST.parse_raw_data_item) ar var);
   implies_trans
-    (cbor_array_iterator_match res (Cbor.Array?.v v))
+    (cbor_array_iterator_match p res (Cbor.Array?.v v))
     (LPS.aparse (LPS.parse_nlist (U64.v res.cbor_array_iterator_length) CborST.parse_raw_data_item) ar var)
-    (raw_data_item_match a v);
+    (raw_data_item_match p a v);
   return res
 
 #pop-options
@@ -1447,7 +1655,7 @@ let cbor_array_iterator_init
   a
 = raw_data_item_match_get_case a;
   match a with
-  | CBOR_Case_Array _ ->
+  | CBOR_Case_Array _ _ ->
     return (cbor_array_iterator_init_array a)
   | _ ->
     return (cbor_array_iterator_init_serialized a)
@@ -1461,164 +1669,171 @@ let cbor_array_iterator_is_done
 #restart-solver
 
 let cbor_array_iterator_next_array
+  (#p: perm)
   (#l: Ghost.erased (list Cbor.raw_data_item))
   (#i1 #i2: Ghost.erased cbor_array_iterator_t)
   (i: cbor_array_iterator_t { i == Ghost.reveal i2 })
   (pi: R.ref cbor_array_iterator_t { Cons? l /\ CBOR_Array_Iterator_Payload_Array? i.cbor_array_iterator_payload })
 : STT cbor
-    (R.pts_to pi full_perm i1 `star` cbor_array_iterator_match i2 l)
+    (R.pts_to pi full_perm i1 `star` cbor_array_iterator_match p i2 l)
     (fun c -> exists_ (fun i' ->
       R.pts_to pi full_perm i' `star`
-      raw_data_item_match c (List.Tot.hd l) `star`
-      cbor_array_iterator_match i' (List.Tot.tl l) `star`
-      ((raw_data_item_match c (List.Tot.hd l) `star`
-        cbor_array_iterator_match i' (List.Tot.tl l)) `implies_`
-        cbor_array_iterator_match i2 l
+      raw_data_item_match p c (List.Tot.hd l) `star`
+      cbor_array_iterator_match p i' (List.Tot.tl l) `star`
+      ((raw_data_item_match p c (List.Tot.hd l) `star`
+        cbor_array_iterator_match p i' (List.Tot.tl l)) `implies_`
+        cbor_array_iterator_match p i2 l
       )
     ))
 = rewrite_with_implies
-    (cbor_array_iterator_match _ l)
-    (cbor_array_iterator_match_array i l);
+    (cbor_array_iterator_match p _ l)
+    (cbor_array_iterator_match_array p i l);
   let _ = gen_elim () in
   let a = CBOR_Array_Iterator_Payload_Array?.payload i.cbor_array_iterator_payload in
   let fp : Ghost.erased _ = CBOR_Array_Iterator_Payload_Array?.footprint i.cbor_array_iterator_payload in
   rewrite
-    (A.pts_to _ full_perm _)
-    (A.pts_to a full_perm fp);
+    (A.pts_to _ p _)
+    (A.pts_to a p fp);
   rewrite
-    (raw_data_item_array_match _ _)
-    (raw_data_item_array_match fp l);
+    (raw_data_item_array_match p _ _)
+    (raw_data_item_array_match p fp l);
   intro_implies
-    (A.pts_to a full_perm fp `star` raw_data_item_array_match fp l)
-    (cbor_array_iterator_match_array i l)
+    ((A.pts_to a p fp `star` GR.pts_to i.footprint p ()) `star` raw_data_item_array_match p fp l)
+    (cbor_array_iterator_match_array p i l)
     emp
     (fun _ -> noop (); noop ());
   implies_trans
-    (A.pts_to a full_perm fp `star` raw_data_item_array_match fp l)
-    (cbor_array_iterator_match_array i l)
-    (cbor_array_iterator_match _ l);
+    ((A.pts_to a p fp `star` GR.pts_to i.footprint p ()) `star` raw_data_item_array_match p fp l)
+    (cbor_array_iterator_match_array p i l)
+    (cbor_array_iterator_match p _ l);
   let len' = i.cbor_array_iterator_length `U64.sub` 1uL in
-  SM.seq_list_match_cons_eq  fp l raw_data_item_match;
+  SM.seq_list_match_cons_eq  fp l (raw_data_item_match p);
   Seq.seq_of_list_tl l;
-  SM.seq_list_match_length raw_data_item_match _ _;
+  SM.seq_list_match_length (raw_data_item_match p) _ _;
   A.pts_to_length _ _;
   rewrite_with_implies
-    (raw_data_item_array_match fp l)
-    (SM.seq_list_match_cons0 fp l raw_data_item_match SM.seq_list_match);
+    (raw_data_item_array_match p fp l)
+    (SM.seq_list_match_cons0 fp l (raw_data_item_match p) SM.seq_list_match);
   implies_trans_r1
-    (A.pts_to _ _ _)
-    (SM.seq_list_match_cons0 fp l raw_data_item_match SM.seq_list_match)
-    (raw_data_item_array_match fp l)
-    (cbor_array_iterator_match _ _);
+    (A.pts_to _ _ _ `star` GR.pts_to _ _ _)
+    (SM.seq_list_match_cons0 fp l (raw_data_item_match p) SM.seq_list_match)
+    (raw_data_item_array_match p fp l)
+    (cbor_array_iterator_match p _ _);
   let _ = gen_elim () in
   let res = A.index a 0sz in
-  vpattern_rewrite (fun c1 -> raw_data_item_match c1 _) res;
-  let c2 = vpattern_replace_erased (fun c2 -> SM.seq_list_match c2 (List.Tot.tl l) raw_data_item_match) in
+  vpattern_rewrite (fun c1 -> raw_data_item_match p c1 _) res;
+  let c2 = vpattern_replace_erased (fun c2 -> SM.seq_list_match c2 (List.Tot.tl l) (raw_data_item_match p)) in
   Seq.lemma_cons_inj (Seq.head fp) res (Seq.tail fp) c2;
   intro_implies
-    (raw_data_item_match res (List.Tot.hd l) `star` SM.seq_list_match c2 (List.Tot.tl l) raw_data_item_match)
-    (SM.seq_list_match_cons0 fp l raw_data_item_match SM.seq_list_match)
+    (raw_data_item_match p res (List.Tot.hd l) `star` SM.seq_list_match c2 (List.Tot.tl l) (raw_data_item_match p))
+    (SM.seq_list_match_cons0 fp l (raw_data_item_match p) SM.seq_list_match)
     emp
     (fun _ -> noop (); noop ());
   rewrite_with_implies
-    (SM.seq_list_match c2 (List.Tot.tl l) raw_data_item_match)
-    (raw_data_item_array_match c2 (List.Tot.tl l));
+    (SM.seq_list_match c2 (List.Tot.tl l) (raw_data_item_match p))
+    (raw_data_item_array_match p c2 (List.Tot.tl l));
   implies_trans_r1
-    (raw_data_item_match res (List.Tot.hd l))
-    (raw_data_item_array_match c2 (List.Tot.tl l))
-    (SM.seq_list_match c2 (List.Tot.tl l) raw_data_item_match)
-    (SM.seq_list_match_cons0 fp l raw_data_item_match SM.seq_list_match);
+    (raw_data_item_match p res (List.Tot.hd l))
+    (raw_data_item_array_match p c2 (List.Tot.tl l))
+    (SM.seq_list_match c2 (List.Tot.tl l) (raw_data_item_match p))
+    (SM.seq_list_match_cons0 fp l (raw_data_item_match p) SM.seq_list_match);
   let _ = A.ghost_split a 1sz in
   let ar' = A.split_r a 1sz in
-  rewrite (A.pts_to (A.split_r _ _) _ _) (A.pts_to ar' full_perm (Ghost.reveal c2));
+  rewrite (A.pts_to (A.split_r _ _) _ _) (A.pts_to ar' p (Ghost.reveal c2));
   intro_implies
-    (A.pts_to ar' full_perm c2)
-    (A.pts_to a full_perm fp)
+    (A.pts_to ar' p c2)
+    (A.pts_to a p fp)
     (A.pts_to (A.split_l _ _) _ _)
     (fun _ ->
       let _ = A.ghost_join (A.split_l _ _) ar' () in
       rewrite
         (A.pts_to _ _ _)
-        (A.pts_to a full_perm fp)
+        (A.pts_to a p fp)
     );
+  implies_reg_r (A.pts_to _ _ _) (A.pts_to _ _ _) (GR.pts_to _ _ _);
   implies_trans_l1
-    (A.pts_to ar' full_perm c2)
-    (A.pts_to a full_perm fp)
-    (SM.seq_list_match_cons0 fp l raw_data_item_match SM.seq_list_match)
-    (cbor_array_iterator_match _ l);
+    (A.pts_to ar' p c2 `star` GR.pts_to _ _ _)
+    (A.pts_to a p fp `star` GR.pts_to _ _ _)
+    (SM.seq_list_match_cons0 fp l (raw_data_item_match p) SM.seq_list_match)
+    (cbor_array_iterator_match p _ l);
   implies_trans_r1
-    (A.pts_to ar' full_perm c2)
-    (raw_data_item_match res (List.Tot.hd l) `star` raw_data_item_array_match c2 (List.Tot.tl l))
-    (SM.seq_list_match_cons0 fp l raw_data_item_match SM.seq_list_match)
-    (cbor_array_iterator_match _ l);
+    (A.pts_to ar' p c2 `star` GR.pts_to _ _ _)
+    (raw_data_item_match p res (List.Tot.hd l) `star` raw_data_item_array_match p c2 (List.Tot.tl l))
+    (SM.seq_list_match_cons0 fp l (raw_data_item_match p) SM.seq_list_match)
+    (cbor_array_iterator_match p _ l);
   implies_with_tactic
-    (raw_data_item_match res (List.Tot.hd l) `star` (A.pts_to ar' full_perm c2 `star` raw_data_item_array_match c2 (List.Tot.tl l)))
-    (A.pts_to ar' full_perm c2 `star` (raw_data_item_match res (List.Tot.hd l) `star` raw_data_item_array_match c2 (List.Tot.tl l)));
+    (raw_data_item_match p res (List.Tot.hd l) `star` (A.pts_to ar' p c2 `star` GR.pts_to i.footprint p () `star` raw_data_item_array_match p c2 (List.Tot.tl l)))
+    ((A.pts_to ar' p c2 `star` GR.pts_to i.footprint p ()) `star` (raw_data_item_match p res (List.Tot.hd l) `star` raw_data_item_array_match p c2 (List.Tot.tl l)));
   implies_trans
-    (raw_data_item_match res (List.Tot.hd l) `star` (A.pts_to ar' full_perm c2 `star` raw_data_item_array_match c2 (List.Tot.tl l)))
-    (A.pts_to ar' full_perm c2 `star` (raw_data_item_match res (List.Tot.hd l) `star` raw_data_item_array_match c2 (List.Tot.tl l)))
-    (cbor_array_iterator_match _ l);
+    (raw_data_item_match p res (List.Tot.hd l) `star` (A.pts_to ar' p c2 `star` GR.pts_to i.footprint p () `star` raw_data_item_array_match p c2 (List.Tot.tl l)))
+    ((A.pts_to ar' p c2 `star` GR.pts_to i.footprint p ()) `star` (raw_data_item_match p res (List.Tot.hd l) `star` raw_data_item_array_match p c2 (List.Tot.tl l)))
+    (cbor_array_iterator_match p _ l);
   let i' = {
     cbor_array_iterator_length = len';
     cbor_array_iterator_payload = CBOR_Array_Iterator_Payload_Array ar' c2;
+    footprint = i.footprint;
   }
   in
   R.write pi i';
+  vpattern_rewrite_with_implies (fun r -> GR.pts_to r _ _) i'.footprint;
   rewrite_with_implies
-    (cbor_array_iterator_match_array i' (List.Tot.tl l))
-    (cbor_array_iterator_match i' (List.Tot.tl l));
+    (cbor_array_iterator_match_array p i' (List.Tot.tl l))
+    (cbor_array_iterator_match p i' (List.Tot.tl l));
   intro_implies
-    (cbor_array_iterator_match_array i' (List.Tot.tl l))
-    (A.pts_to ar' full_perm c2 `star` raw_data_item_array_match c2 (List.Tot.tl l))
-    emp
+    (cbor_array_iterator_match_array p i' (List.Tot.tl l))
+    (A.pts_to ar' p c2 `star` GR.pts_to i.footprint p () `star`  raw_data_item_array_match p c2 (List.Tot.tl l))
+    (GR.pts_to i'.footprint p () `implies_` GR.pts_to i.footprint p ())
     (fun _ ->
       let _ = gen_elim () in
-      rewrite (A.pts_to _ _ _) (A.pts_to ar' full_perm c2);
-      rewrite (raw_data_item_array_match _ _) (raw_data_item_array_match c2 (List.Tot.tl l))
+      elim_implies (GR.pts_to i'.footprint p ()) (GR.pts_to i.footprint p ());
+      rewrite (A.pts_to _ _ _) (A.pts_to ar' p c2);
+      rewrite (raw_data_item_array_match p _ _) (raw_data_item_array_match p c2 (List.Tot.tl l))
     );
   implies_trans
-    (cbor_array_iterator_match i' (List.Tot.tl l))
-    (cbor_array_iterator_match_array i' (List.Tot.tl l))
-    (A.pts_to ar' full_perm c2 `star` raw_data_item_array_match c2 (List.Tot.tl l));
+    (cbor_array_iterator_match p i' (List.Tot.tl l))
+    (cbor_array_iterator_match_array p i' (List.Tot.tl l))
+    (A.pts_to ar' p c2 `star` GR.pts_to i.footprint p () `star` raw_data_item_array_match p c2 (List.Tot.tl l));
   implies_trans_r1
-    (raw_data_item_match res (List.Tot.hd l))
-    (cbor_array_iterator_match i' (List.Tot.tl l))
-    (A.pts_to ar' full_perm c2 `star` raw_data_item_array_match c2 (List.Tot.tl l))
-    (cbor_array_iterator_match _ l);
+    (raw_data_item_match p res (List.Tot.hd l))
+    (cbor_array_iterator_match p i' (List.Tot.tl l))
+    (A.pts_to ar' p c2 `star` GR.pts_to i.footprint p () `star` raw_data_item_array_match p c2 (List.Tot.tl l))
+    (cbor_array_iterator_match p _ l);
   return res
 
 let cbor_array_iterator_next_serialized
+  (#p: perm)
   (#l: Ghost.erased (list Cbor.raw_data_item))
   (#i1 #i2: Ghost.erased cbor_array_iterator_t)
   (i: cbor_array_iterator_t { i == Ghost.reveal i2 })
   (pi: R.ref cbor_array_iterator_t { Cons? l /\ CBOR_Array_Iterator_Payload_Serialized? i.cbor_array_iterator_payload })
 : STT cbor
-    (R.pts_to pi full_perm i1 `star` cbor_array_iterator_match i2 l)
+    (R.pts_to pi full_perm i1 `star` cbor_array_iterator_match p i2 l)
     (fun c -> exists_ (fun i' ->
       R.pts_to pi full_perm i' `star`
-      raw_data_item_match c (List.Tot.hd l) `star`
-      cbor_array_iterator_match i' (List.Tot.tl l) `star`
-      ((raw_data_item_match c (List.Tot.hd l) `star`
-        cbor_array_iterator_match i' (List.Tot.tl l)) `implies_`
-        cbor_array_iterator_match i2 l
+      raw_data_item_match p c (List.Tot.hd l) `star`
+      cbor_array_iterator_match p i' (List.Tot.tl l) `star`
+      ((raw_data_item_match p c (List.Tot.hd l) `star`
+        cbor_array_iterator_match p i' (List.Tot.tl l)) `implies_`
+        cbor_array_iterator_match p i2 l
       )
     ))
 = rewrite_with_implies
-    (cbor_array_iterator_match _ l)
-    (cbor_array_iterator_match_serialized i l);
+    (cbor_array_iterator_match p _ l)
+    (cbor_array_iterator_match_serialized p i l);
   let _ = gen_elim () in
+  GR.pts_to_perm i.footprint;
   let a = CBOR_Array_Iterator_Payload_Serialized?.payload i.cbor_array_iterator_payload in
   let va = vpattern_replace (LPS.aparse (LPS.parse_nlist (U64.v i.cbor_array_iterator_length) CborST.parse_raw_data_item) _) in
   vpattern_rewrite (fun a -> LPS.aparse (LPS.parse_nlist (U64.v i.cbor_array_iterator_length) CborST.parse_raw_data_item) a _) a;
   intro_implies
-    (LPS.aparse (LPS.parse_nlist (U64.v i.cbor_array_iterator_length) CborST.parse_raw_data_item) a va)
-    (cbor_array_iterator_match_serialized i l)
+    (LPS.aparse (LPS.parse_nlist (U64.v i.cbor_array_iterator_length) CborST.parse_raw_data_item) a va `star` GR.pts_to i.footprint p ())
+    (cbor_array_iterator_match_serialized p i l)
     emp
     (fun _ -> noop (); noop ());
   implies_trans
-    (LPS.aparse (LPS.parse_nlist (U64.v i.cbor_array_iterator_length) CborST.parse_raw_data_item) a va)
-    (cbor_array_iterator_match_serialized i l)
-    (cbor_array_iterator_match i2 l);
+    (LPS.aparse (LPS.parse_nlist (U64.v i.cbor_array_iterator_length) CborST.parse_raw_data_item) a va `star` GR.pts_to i.footprint p ())
+    (cbor_array_iterator_match_serialized p i l)
+    (cbor_array_iterator_match p i2 l);
   let len' = i.cbor_array_iterator_length `U64.sub` 1uL in
   let ga' = LPS.elim_nlist_cons
     CborST.parse_raw_data_item
@@ -1641,39 +1856,54 @@ let cbor_array_iterator_next_serialized
         (LPS.aparse (LPS.parse_nlist (U64.v i.cbor_array_iterator_length) CborST.parse_raw_data_item) a)
         va
     );
-  implies_trans
+  implies_trans_l1
     (LPS.aparse CborST.parse_raw_data_item a vl `star` LPS.aparse (LPS.parse_nlist (U64.v len') CborST.parse_raw_data_item) a' va1)
     (LPS.aparse (LPS.parse_nlist (U64.v i.cbor_array_iterator_length) CborST.parse_raw_data_item) a va)
-    (cbor_array_iterator_match i2 l);
-  let res = read_valid_cbor_from_buffer_with_size_strong a sz in
-  vpattern_rewrite_with_implies (raw_data_item_match res) (List.Tot.hd l);
+    (GR.pts_to i.footprint p ())
+    (cbor_array_iterator_match p i2 l);
+  implies_with_tactic
+    (LPS.aparse CborST.parse_raw_data_item a vl `star` (LPS.aparse (LPS.parse_nlist (U64.v len') CborST.parse_raw_data_item) a' va1 `star` GR.pts_to i.footprint p ()))
+    ((LPS.aparse CborST.parse_raw_data_item a vl `star` LPS.aparse (LPS.parse_nlist (U64.v len') CborST.parse_raw_data_item) a' va1) `star` GR.pts_to i.footprint p ());
   implies_trans
-    (raw_data_item_match res (List.Tot.hd l))
-    (raw_data_item_match res _)
+    (LPS.aparse CborST.parse_raw_data_item a vl `star` (LPS.aparse (LPS.parse_nlist (U64.v len') CborST.parse_raw_data_item) a' va1 `star` GR.pts_to i.footprint p ()))
+    ((LPS.aparse CborST.parse_raw_data_item a vl `star` LPS.aparse (LPS.parse_nlist (U64.v len') CborST.parse_raw_data_item) a' va1) `star` GR.pts_to i.footprint p ())
+    (cbor_array_iterator_match p i2 l);
+  let res = read_valid_cbor_from_buffer_with_size_strong p a sz in
+  vpattern_rewrite_with_implies (raw_data_item_match p res) (List.Tot.hd l);
+  implies_trans
+    (raw_data_item_match p res (List.Tot.hd l))
+    (raw_data_item_match p res _)
     (LPS.aparse CborST.parse_raw_data_item a vl);
   implies_trans_l1
-    (raw_data_item_match res (List.Tot.hd l))
+    (raw_data_item_match p res (List.Tot.hd l))
     (LPS.aparse CborST.parse_raw_data_item a vl)
-    (LPS.aparse (LPS.parse_nlist (U64.v len') CborST.parse_raw_data_item) a' va1)
-    (cbor_array_iterator_match i2 l);
+    (LPS.aparse (LPS.parse_nlist (U64.v len') CborST.parse_raw_data_item) a' va1 `star` GR.pts_to i.footprint p ())
+    (cbor_array_iterator_match p i2 l);
   let i' = {
     cbor_array_iterator_length = len';
-    cbor_array_iterator_payload = CBOR_Array_Iterator_Payload_Serialized a' (LPS.array_of va1);
+    cbor_array_iterator_payload = CBOR_Array_Iterator_Payload_Serialized a' (LPA.set_array_perm (LPS.array_of va1) (LPA.array_perm (LPS.array_of va1) `div_perm` p));
+    footprint = i.footprint;
   }
   in
   R.write pi i';
+  vpattern_rewrite_with_implies (fun r -> GR.pts_to r _ _) i'.footprint;
   let va' = LPS.rewrite_aparse_with_implies a' (LPS.parse_nlist (U64.v i'.cbor_array_iterator_length) CborST.parse_raw_data_item) in
-  implies_trans_r1
-    (raw_data_item_match res (List.Tot.hd l))
+  implies_join
     (LPS.aparse (LPS.parse_nlist (U64.v i'.cbor_array_iterator_length) CborST.parse_raw_data_item) a' va')
     (LPS.aparse (LPS.parse_nlist (U64.v len') CborST.parse_raw_data_item) a' va1)
-    (cbor_array_iterator_match i2 l);
+    (GR.pts_to i'.footprint p ())
+    (GR.pts_to i.footprint p ());
+  implies_trans_r1
+    (raw_data_item_match p res (List.Tot.hd l))
+    (LPS.aparse (LPS.parse_nlist (U64.v i'.cbor_array_iterator_length) CborST.parse_raw_data_item) a' va' `star` GR.pts_to i'.footprint p ())
+    (LPS.aparse (LPS.parse_nlist (U64.v len') CborST.parse_raw_data_item) a' va1 `star` GR.pts_to i.footprint p ())
+    (cbor_array_iterator_match p i2 l);
   rewrite_with_implies
-    (cbor_array_iterator_match_serialized i' (List.Tot.tl l))
-    (cbor_array_iterator_match i' (List.Tot.tl l));
+    (cbor_array_iterator_match_serialized p i' (List.Tot.tl l))
+    (cbor_array_iterator_match p i' (List.Tot.tl l));
   intro_implies
-    (cbor_array_iterator_match_serialized i' (List.Tot.tl l))
-    (LPS.aparse (LPS.parse_nlist (U64.v i'.cbor_array_iterator_length) CborST.parse_raw_data_item) a' va')
+    (cbor_array_iterator_match_serialized p i' (List.Tot.tl l))
+    (LPS.aparse (LPS.parse_nlist (U64.v i'.cbor_array_iterator_length) CborST.parse_raw_data_item) a' va' `star` GR.pts_to i'.footprint p ())
     emp
     (fun _ ->
       let _ = gen_elim () in
@@ -1682,14 +1912,14 @@ let cbor_array_iterator_next_serialized
         (LPS.aparse (LPS.parse_nlist (U64.v i'.cbor_array_iterator_length) CborST.parse_raw_data_item) a' va')
     );
   implies_trans
-    (cbor_array_iterator_match i' (List.Tot.tl l))
-    (cbor_array_iterator_match_serialized i' (List.Tot.tl l))
-    (LPS.aparse (LPS.parse_nlist (U64.v i'.cbor_array_iterator_length) CborST.parse_raw_data_item) a' va');
+    (cbor_array_iterator_match p i' (List.Tot.tl l))
+    (cbor_array_iterator_match_serialized p i' (List.Tot.tl l))
+    (LPS.aparse (LPS.parse_nlist (U64.v i'.cbor_array_iterator_length) CborST.parse_raw_data_item) a' va' `star` GR.pts_to i'.footprint p ());
   implies_trans_r1
-    (raw_data_item_match res (List.Tot.hd l))
-    (cbor_array_iterator_match i' (List.Tot.tl l))
-    (LPS.aparse (LPS.parse_nlist (U64.v i'.cbor_array_iterator_length) CborST.parse_raw_data_item) a' va')
-    (cbor_array_iterator_match i2 l);
+    (raw_data_item_match p res (List.Tot.hd l))
+    (cbor_array_iterator_match p i' (List.Tot.tl l))
+    (LPS.aparse (LPS.parse_nlist (U64.v i'.cbor_array_iterator_length) CborST.parse_raw_data_item) a' va' `star` GR.pts_to i'.footprint p ())
+    (cbor_array_iterator_match p i2 l);
   return res
 
 #pop-options
@@ -1706,6 +1936,7 @@ let cbor_array_iterator_next
 inline_for_extraction
 noextract
 let read_cbor_array_payload
+  (p: perm)
   (n0: U64.t)
   (vl0: LPS.v (LowParse.Spec.VCList.parse_nlist_kind (U64.v n0) CborST.parse_raw_data_item_kind) (LowParse.Spec.VCList.nlist (U64.v n0) Cbor.raw_data_item))
   (l0: LPS.byte_array)
@@ -1717,57 +1948,91 @@ let read_cbor_array_payload
     )
     (fun res ->
       A.pts_to a0 full_perm res `star`
-      raw_data_item_array_match res vl0.contents `star`
-      (raw_data_item_array_match res vl0.contents `implies_`
+      raw_data_item_array_match p res vl0.contents `star`
+      (raw_data_item_array_match p res vl0.contents `implies_`
         LPS.aparse (LowParse.Spec.VCList.parse_nlist (U64.v n0) CborST.parse_raw_data_item) l0 vl0
       )
     )
     (A.length a0 == U64.v n0 /\
+      p `lesser_equal_perm` full_perm /\
       SZ.fits_u64
     )
     (fun _ -> True)
 =
   let n0_as_sz = SZ.uint64_to_sizet n0 in
   let vl = LPS.rewrite_aparse_with_implies l0 (LPS.parse_nlist (SZ.v n0_as_sz) CborST.parse_raw_data_item) in
-  let res = LPS.read_array_payload_from_nlist CborST.jump_raw_data_item raw_data_item_match (fun a alen -> read_valid_cbor_from_buffer_with_size_strong a alen) n0_as_sz l0 a0 in
+  let res = LPS.read_array_payload_from_nlist CborST.jump_raw_data_item (raw_data_item_match p) (fun a alen -> read_valid_cbor_from_buffer_with_size_strong p a alen) n0_as_sz l0 a0 in
   implies_trans
-    (LPS.seq_list_match res vl.contents raw_data_item_match)
+    (LPS.seq_list_match res vl.contents (raw_data_item_match p))
     (LPS.aparse (LowParse.Spec.VCList.parse_nlist (SZ.v n0_as_sz) CborST.parse_raw_data_item) l0 vl)
     (LPS.aparse (LowParse.Spec.VCList.parse_nlist (U64.v n0) CborST.parse_raw_data_item) l0 vl0);
   rewrite_with_implies_with_tactic
-    (LPS.seq_list_match res vl.contents raw_data_item_match)
-    (raw_data_item_array_match res vl.contents);
+    (LPS.seq_list_match res vl.contents (raw_data_item_match p))
+    (raw_data_item_array_match p res vl.contents);
   implies_trans
-    (raw_data_item_array_match res vl.contents)
-    (LPS.seq_list_match res vl.contents raw_data_item_match)
+    (raw_data_item_array_match p res vl.contents)
+    (LPS.seq_list_match res vl.contents (raw_data_item_match p))
     (LPS.aparse (LowParse.Spec.VCList.parse_nlist (U64.v n0) CborST.parse_raw_data_item) l0 vl0);
   rewrite_with_implies
-    (raw_data_item_array_match res vl.contents)
-    (raw_data_item_array_match res vl0.contents);
+    (raw_data_item_array_match p res vl.contents)
+    (raw_data_item_array_match p res vl0.contents);
   implies_trans
-    (raw_data_item_array_match res vl0.contents)
-    (raw_data_item_array_match res vl.contents)
+    (raw_data_item_array_match p res vl0.contents)
+    (raw_data_item_array_match p res vl.contents)
     (LPS.aparse (LowParse.Spec.VCList.parse_nlist (U64.v n0) CborST.parse_raw_data_item) l0 vl0);
   return res
+
+let array_lower_perm
+  (#t: Type)
+  (#opened: _)
+  (#high: perm)
+  (#v: Seq.seq t)
+  (r: A.array t)
+  (low: perm)
+: STGhost unit opened
+    (A.pts_to r high v)
+    (fun _ -> A.pts_to r low v `star`
+      (A.pts_to r low v `implies_` A.pts_to r high v)
+    )
+    (low `lesser_equal_perm` high)
+    (fun _ -> True)
+= if FStar.StrongExcludedMiddle.strong_excluded_middle (low == high)
+  then
+    vpattern_rewrite_with_implies
+      (fun p -> A.pts_to _ p _)
+      low
+  else begin
+    let diff = diff_perm high low in
+    A.share r high low diff;
+    intro_implies
+      (A.pts_to r low v)
+      (A.pts_to r high v)
+      (A.pts_to r diff v)
+      (fun _ ->
+        A.gather r low diff;
+        vpattern_rewrite (fun p -> A.pts_to _ p _) high
+      )
+  end
 
 #push-options "--z3rlimit 64"
 #restart-solver
 
 let read_cbor_array
-  #obj input a0 len
+  #p #obj input a0 len
 = 
+  raw_data_item_match_perm_le_full_perm input;
   A.pts_to_length a0 _;
   raw_data_item_match_get_case input;
   match input with
-  | CBOR_Case_Array _ ->
+  | CBOR_Case_Array _ _ ->
     let res = destr_cbor_array input in
     A.pts_to_length res.cbor_array_payload _;
-    SM.seq_list_match_length raw_data_item_match res.footprint (maybe_cbor_array obj);
+    SM.seq_list_match_length (raw_data_item_match p) res.footprint (maybe_cbor_array obj);
     implies_concl_r
-      (A.pts_to _ _ _ `star` raw_data_item_array_match _ _)
-      (raw_data_item_match _ _)
+      (A.pts_to _ _ _ `star` raw_data_item_array_match p _ _)
+      (raw_data_item_match p _ _)
       (exists_ (A.pts_to a0 full_perm));
-    return res
+    return res.cbor_array_payload
   | _ ->
     let s = destr_cbor_serialized input in
     let _ = gen_elim () in
@@ -1776,31 +2041,22 @@ let read_cbor_array
     implies_trans
       (LPS.aparse (LowParse.Spec.VCList.parse_nlist (U64.v len) CborST.parse_raw_data_item) a _)
       (LPS.aparse CborST.parse_raw_data_item s.cbor_serialized_payload _)
-      (raw_data_item_match input _);
+      (raw_data_item_match p input _);
     let _ = A.intro_fits_u64 () in
-    let va = read_cbor_array_payload len _ a a0 in
+    let va = read_cbor_array_payload p len _ a a0 in
     implies_trans
-      (raw_data_item_array_match va _)
+      (raw_data_item_array_match p va _)
       (LPS.aparse (LowParse.Spec.VCList.parse_nlist (U64.v len) CborST.parse_raw_data_item) a _)
-      (raw_data_item_match input _);
-    [@@inline_let]
-    let res = {
-      cbor_array_length = len;
-      cbor_array_payload = a0;
-      footprint = va;
-    }
-    in
+      (raw_data_item_match p input _);
     rewrite_with_implies
-      (raw_data_item_array_match _ _)
-      (raw_data_item_array_match res.footprint (maybe_cbor_array obj));
-    SM.seq_list_match_length raw_data_item_match res.footprint (maybe_cbor_array obj);
+      (raw_data_item_array_match p _ _)
+      (raw_data_item_array_match p va (maybe_cbor_array obj));
+    SM.seq_list_match_length (raw_data_item_match p) va (maybe_cbor_array obj);
     implies_trans
-      (raw_data_item_array_match res.footprint (maybe_cbor_array obj))
-      (raw_data_item_array_match _ _)
-      (raw_data_item_match input _);
-    rewrite_with_implies
-      (A.pts_to _ _ _)
-      (A.pts_to res.cbor_array_payload full_perm res.footprint);
+      (raw_data_item_array_match p va (maybe_cbor_array obj))
+      (raw_data_item_array_match p _ _)
+      (raw_data_item_match p input _);
+    array_lower_perm a0 p;
     intro_implies
       (A.pts_to a0 full_perm va)
       (exists_ (A.pts_to a0 full_perm))
@@ -1813,13 +2069,13 @@ let read_cbor_array
     implies_join
       (A.pts_to _ _ _)
       (exists_ (A.pts_to _ _))
-      (raw_data_item_array_match _ _)
-      (raw_data_item_match _ _);
+      (raw_data_item_array_match p _ _)
+      (raw_data_item_match p _ _);
     implies_swap_r
-      (A.pts_to _ _ _ `star` raw_data_item_array_match _ _)
+      (A.pts_to _ _ _ `star` raw_data_item_array_match p _ _)
       (exists_ (A.pts_to _ _))
-      (raw_data_item_match _ _);
-    return res
+      (raw_data_item_match p _ _);
+    return a0
 
 #pop-options
 
@@ -1861,7 +2117,7 @@ let size_comp_for_array
   (va: Ghost.erased Cbor.raw_data_item)
   (c: cbor {CBOR_Case_Array? c})
 : Tot (cbor_size_comp_for va c)
-= fun sz perr ->
+= fun #p sz perr ->
     let _ = A.intro_fits_u64 () in
     raw_data_item_match_get_case c;
     let _ : squash (Cbor.Array? va) = () in
@@ -1870,14 +2126,14 @@ let size_comp_for_array
     let l = Ghost.hide (maybe_cbor_array va) in
     assert (Ghost.reveal l == Cbor.Array?.v va);
     rewrite_with_implies_with_tactic
-      (raw_data_item_array_match _ _)
-      (LPS.seq_list_match c'.footprint l raw_data_item_match);
+      (raw_data_item_array_match p _ _)
+      (LPS.seq_list_match c'.footprint l (raw_data_item_match p));
     implies_trans_r1
       (A.pts_to _ _ _)
-      (LPS.seq_list_match c'.footprint l raw_data_item_match)
-      (raw_data_item_array_match _ _)
-      (raw_data_item_match _ _);
-    LPS.seq_list_match_length raw_data_item_match _ _;
+      (LPS.seq_list_match c'.footprint l (raw_data_item_match p))
+      (raw_data_item_array_match p _ _)
+      (raw_data_item_match p _ _);
+    LPS.seq_list_match_length (raw_data_item_match p) _ _;
     A.pts_to_length _ _;
     let sz1 = CBOR.SteelST.Raw.Write.size_comp_uint64_header Cbor.major_type_array c'.cbor_array_length sz perr in
     let _ = gen_elim () in
@@ -1886,14 +2142,14 @@ let size_comp_for_array
     then begin
       noop ();
       elim_implies
-        (A.pts_to _ _ _ `star` LPS.seq_list_match c'.footprint l raw_data_item_match)
-        (raw_data_item_match _ _);
+        (A.pts_to _ _ _ `star` LPS.seq_list_match c'.footprint l (raw_data_item_match p))
+        (raw_data_item_match p _ _);
       return sz1
     end else begin
       noop ();
       let sz2 = LPS.array_payload_as_nlist_size
         CborST.serialize_raw_data_item
-        raw_data_item_match
+        (raw_data_item_match p)
         (fun x y sz perr ->
           let res = size y x sz perr in
           let _ = gen_elim () in
@@ -1908,8 +2164,8 @@ let size_comp_for_array
       in
       let _ = gen_elim () in
       elim_implies
-        (A.pts_to _ _ _ `star` LPS.seq_list_match c'.footprint l raw_data_item_match)
-        (raw_data_item_match _ _);
+        (A.pts_to _ _ _ `star` LPS.seq_list_match c'.footprint l (raw_data_item_match p))
+        (raw_data_item_match p _ _);
       return sz2
     end
 
@@ -1926,7 +2182,7 @@ let l2r_writer_for_array
   (va: Ghost.erased Cbor.raw_data_item)
   (c: cbor {CBOR_Case_Array? c})
 : Tot (cbor_l2r_writer_for va c)
-= fun #vout out ->
+= fun #p #vout out ->
     let _ = A.intro_fits_u64 () in
     raw_data_item_match_get_case c;
     let _ : squash (Cbor.Array? va) = () in
@@ -1935,21 +2191,21 @@ let l2r_writer_for_array
     let l = Ghost.hide (maybe_cbor_array va) in
     assert (Ghost.reveal l == Cbor.Array?.v va);
     rewrite_with_implies_with_tactic
-      (raw_data_item_array_match _ _)
-      (LPS.seq_list_match c'.footprint l raw_data_item_match);
+      (raw_data_item_array_match p _ _)
+      (LPS.seq_list_match c'.footprint l (raw_data_item_match p));
     implies_trans_r1
       (A.pts_to _ _ _)
-      (LPS.seq_list_match c'.footprint l raw_data_item_match)
-      (raw_data_item_array_match _ _)
-      (raw_data_item_match _ _);
-    LPS.seq_list_match_length raw_data_item_match _ _;
+      (LPS.seq_list_match c'.footprint l (raw_data_item_match p))
+      (raw_data_item_array_match p _ _)
+      (raw_data_item_match p _ _);
+    LPS.seq_list_match_length (raw_data_item_match p) _ _;
     A.pts_to_length _ _;
     let res = CBOR.SteelST.Raw.Write.l2r_write_uint64_header Cbor.major_type_array c'.cbor_array_length out in
     let _ = gen_elim () in
     let _ = LPS.elim_aparse_with_serializer CborST.serialize_header res in
     let res_pl = LPS.l2r_write_array_payload_as_nlist
       CborST.serialize_raw_data_item
-      raw_data_item_match
+      (raw_data_item_match p)
       (fun x y out ->
          let res = write y x out in
          let _ = gen_elim () in
@@ -1968,31 +2224,32 @@ let l2r_writer_for_array
     let _ = gen_elim () in
     let vres = LPS.intro_aparse_with_serializer CborST.serialize_raw_data_item va res in
     elim_implies
-      (A.pts_to _ _ _ `star` LPS.seq_list_match c'.footprint l raw_data_item_match)
-      (raw_data_item_match _ _);
-    assert_ (cbor_l2r_writer_for_post va c vout out res vres vout'); // FIXME: WHY WHY WHY?
+      (A.pts_to _ _ _ `star` LPS.seq_list_match c'.footprint l (raw_data_item_match p))
+      (raw_data_item_match p _ _);
+    assert_ (cbor_l2r_writer_for_post p va c vout out res vres vout'); // FIXME: WHY WHY WHY?
     return res
 
 #pop-options
 
-let destr_cbor_tagged
+let destr_cbor_tagged0
+  (#p: perm)
   (#v: Ghost.erased Cbor.raw_data_item)
   (a: cbor)
-: ST cbor_tagged
-    (raw_data_item_match a v)
+: ST cbor_tagged0
+    (raw_data_item_match p a v)
     (fun res ->
-      R.pts_to res.cbor_tagged_payload full_perm res.footprint `star`
-      raw_data_item_match res.footprint (maybe_cbor_tagged_payload v) `star`
-      ((R.pts_to res.cbor_tagged_payload full_perm res.footprint `star`
-        raw_data_item_match res.footprint (maybe_cbor_tagged_payload v)) `implies_`
-        raw_data_item_match a v
+      R.pts_to res.cbor_tagged0_payload p res.footprint `star`
+      raw_data_item_match p res.footprint (maybe_cbor_tagged_payload v) `star`
+      ((R.pts_to res.cbor_tagged0_payload p res.footprint `star`
+        raw_data_item_match p res.footprint (maybe_cbor_tagged_payload v)) `implies_`
+        raw_data_item_match p a v
       )
     )
     (CBOR_Case_Tagged? a)
     (fun res ->
       a == CBOR_Case_Tagged res /\
       Cbor.Tagged? v /\
-      res.cbor_tagged_tag == Cbor.Tagged?.tag v
+      res.cbor_tagged0_tag == Cbor.Tagged?.tag v
     )
 = raw_data_item_match_get_case _;
   let _ : squash (Cbor.Tagged? v) = () in
@@ -2000,39 +2257,121 @@ let destr_cbor_tagged
   let g_payload = Ghost.hide (Cbor.Tagged?.v v) in
   let CBOR_Case_Tagged res = a in
   rewrite_with_implies
-    (raw_data_item_match a v)
-    (raw_data_item_match (CBOR_Case_Tagged res) (Cbor.Tagged g_tag g_payload));
+    (raw_data_item_match p a v)
+    (raw_data_item_match p (CBOR_Case_Tagged res) (Cbor.Tagged g_tag g_payload));
   rewrite_with_implies_with_tactic
-    (raw_data_item_match (CBOR_Case_Tagged res) (Cbor.Tagged g_tag g_payload))
-    (raw_data_item_match_tagged0 (CBOR_Case_Tagged res) (Cbor.Tagged g_tag g_payload) raw_data_item_match);
+    (raw_data_item_match p (CBOR_Case_Tagged res) (Cbor.Tagged g_tag g_payload))
+    (raw_data_item_match_tagged0 p (CBOR_Case_Tagged res) (Cbor.Tagged g_tag g_payload) (raw_data_item_match p));
   implies_trans
-    (raw_data_item_match_tagged0 (CBOR_Case_Tagged res) (Cbor.Tagged g_tag g_payload) raw_data_item_match)
-    (raw_data_item_match (CBOR_Case_Tagged res) (Cbor.Tagged g_tag g_payload))
-    (raw_data_item_match a v);
+    (raw_data_item_match_tagged0 p (CBOR_Case_Tagged res) (Cbor.Tagged g_tag g_payload) (raw_data_item_match p))
+    (raw_data_item_match p (CBOR_Case_Tagged res) (Cbor.Tagged g_tag g_payload))
+    (raw_data_item_match p a v);
   let _ = gen_elim () in
-  let _ : squash (res.cbor_tagged_tag == Ghost.reveal g_tag) = () in
+  let _ : squash (res.cbor_tagged0_tag == Ghost.reveal g_tag) = () in
   let _ : squash (maybe_cbor_tagged_payload v == Ghost.reveal g_payload) = () in
   let _ : squash (Ghost.reveal g_payload << Cbor.Tagged g_tag g_payload) = () in // FIXME: WHY WHY WHY?
-  rewrite (R.pts_to _ _ _) (R.pts_to res.cbor_tagged_payload full_perm res.footprint);
-  rewrite (raw_data_item_match _ _) (raw_data_item_match res.footprint (maybe_cbor_tagged_payload v));
+  rewrite (R.pts_to _ _ _) (R.pts_to res.cbor_tagged0_payload p res.footprint);
+  rewrite (raw_data_item_match p _ _) (raw_data_item_match p res.footprint (maybe_cbor_tagged_payload v));
   intro_implies
-    (R.pts_to res.cbor_tagged_payload full_perm res.footprint `star`
-      raw_data_item_match res.footprint (maybe_cbor_tagged_payload v))
-    (raw_data_item_match a v)
-    (raw_data_item_match_tagged0 _ _ raw_data_item_match `implies_` raw_data_item_match a _)
+    (R.pts_to res.cbor_tagged0_payload p res.footprint `star`
+      raw_data_item_match p res.footprint (maybe_cbor_tagged_payload v))
+    (raw_data_item_match p a v)
+    (raw_data_item_match_tagged0 p _ _ (raw_data_item_match p) `implies_` raw_data_item_match p a _)
     (fun _ ->
       elim_implies
-        (raw_data_item_match_tagged0 (CBOR_Case_Tagged res) (Cbor.Tagged g_tag g_payload) raw_data_item_match)
-        (raw_data_item_match a _)
+        (raw_data_item_match_tagged0 p (CBOR_Case_Tagged res) (Cbor.Tagged g_tag g_payload) (raw_data_item_match p))
+        (raw_data_item_match p a _)
     );
   return res
+
+let implies_consumes_l
+  (#opened: _)
+  (p q r: vprop)
+: STGhostT unit opened
+    (p `star` ((p `star` q) `implies_` r))
+    (fun _ -> q `implies_` r)
+= intro_implies
+    q
+    r
+    (p `star` ((p `star` q) `implies_` r))
+    (fun _ -> elim_implies (p `star` q) r)
+
+let implies_consumes_r
+  (#opened: _)
+  (p q r: vprop)
+: STGhostT unit opened
+    (q `star` ((p `star` q) `implies_` r))
+    (fun _ -> p `implies_` r)
+= implies_with_tactic (q `star` p) (p `star` q);
+  implies_trans (q `star` p) (p `star` q) r;
+  implies_consumes_l q p r
+
+#push-options "--z3rlimit 64"
+#restart-solver
+
+let destr_cbor_tagged
+  #p #v a
+=
+  raw_data_item_match_get_case a;
+  match a with
+  | CBOR_Case_Tagged _ ->
+    let r = destr_cbor_tagged0 a in
+    let pl = R.read r.cbor_tagged0_payload in
+    implies_consumes_l
+      (R.pts_to _ _ _)
+      (raw_data_item_match _ _ _)
+      (raw_data_item_match _ _ _);
+    let res = {
+      cbor_tagged_tag = r.cbor_tagged0_tag;
+      cbor_tagged_payload = pl;
+    }
+    in
+    vpattern_rewrite_with_implies
+      (fun pl -> raw_data_item_match p pl _)
+      res.cbor_tagged_payload;
+    implies_trans
+      (raw_data_item_match p _ (maybe_cbor_tagged_payload v))
+      (raw_data_item_match p _ (maybe_cbor_tagged_payload v))
+      (raw_data_item_match p a v);
+    return res
+  | _ ->
+    raw_data_item_match_perm_le_full_perm a;
+    let s = destr_cbor_serialized a in
+    let _ = gen_elim () in
+    let tag = CBOR.SteelST.Raw.read_argument_as_uint64 s.cbor_serialized_payload in
+    let s' = CBOR.SteelST.Raw.Read.focus_tagged s.cbor_serialized_payload in
+    let _ = gen_elim () in
+    implies_trans
+      (LPS.aparse CborST.parse_raw_data_item _ _)
+      (LPS.aparse CborST.parse_raw_data_item _ _)
+      (raw_data_item_match p _ _);
+    let sz = LPS.get_parsed_size CborST.jump_raw_data_item s' in
+    let pl = read_valid_cbor_from_buffer_with_size_strong p s' sz in
+    implies_trans
+      (raw_data_item_match p _ _)
+      (LPS.aparse CborST.parse_raw_data_item _ _)
+      (raw_data_item_match p _ _);
+    [@@inline_let]
+    let res = {
+      cbor_tagged_tag = tag;
+      cbor_tagged_payload = pl;
+    }
+    in
+    rewrite_with_implies
+      (raw_data_item_match p _ _)
+      (raw_data_item_match p res.cbor_tagged_payload (maybe_cbor_tagged_payload v));
+    implies_trans
+      (raw_data_item_match p res.cbor_tagged_payload (maybe_cbor_tagged_payload v))
+      (raw_data_item_match p _ _)
+      (raw_data_item_match p a v);
+    return res
 
 let constr_cbor_tagged
   #c' #v' tag a
 = [@@inline_let]
   let res_tg = {
-    cbor_tagged_tag = tag;
-    cbor_tagged_payload = a;
+    cbor_tagged0_tag = tag;
+    cbor_tagged0_payload = a;
     footprint = c';
   }
   in
@@ -2046,12 +2385,12 @@ let constr_cbor_tagged
   let _ = prf () in
   noop ();
   rewrite_with_implies_with_tactic
-    (raw_data_item_match_tagged0 (CBOR_Case_Tagged res_tg) (Cbor.Tagged tag v') raw_data_item_match)
-    (raw_data_item_match (CBOR_Case_Tagged res_tg) (Cbor.Tagged tag v'));
+    (raw_data_item_match_tagged0 full_perm (CBOR_Case_Tagged res_tg) (Cbor.Tagged tag v') (raw_data_item_match full_perm))
+    (raw_data_item_match full_perm (CBOR_Case_Tagged res_tg) (Cbor.Tagged tag v'));
   intro_implies
-    (raw_data_item_match_tagged0 (CBOR_Case_Tagged res_tg) (Cbor.Tagged tag v') raw_data_item_match)
+    (raw_data_item_match_tagged0 full_perm (CBOR_Case_Tagged res_tg) (Cbor.Tagged tag v') (raw_data_item_match full_perm))
     (R.pts_to a full_perm c' `star`
-      raw_data_item_match c' v')
+      raw_data_item_match full_perm c' v')
     emp
     (fun _ ->
       let _ = gen_elim () in
@@ -2059,94 +2398,25 @@ let constr_cbor_tagged
         (R.pts_to _ _ _)
         (R.pts_to a full_perm c');
       rewrite
-        (raw_data_item_match _ _)
-        (raw_data_item_match c' v')
+        (raw_data_item_match full_perm _ _)
+        (raw_data_item_match full_perm c' v')
     );
   implies_trans
-    (raw_data_item_match (CBOR_Case_Tagged res_tg) (Cbor.Tagged tag v'))
-    (raw_data_item_match_tagged0 (CBOR_Case_Tagged res_tg) (Cbor.Tagged tag v') raw_data_item_match)
+    (raw_data_item_match full_perm (CBOR_Case_Tagged res_tg) (Cbor.Tagged tag v'))
+    (raw_data_item_match_tagged0 full_perm (CBOR_Case_Tagged res_tg) (Cbor.Tagged tag v') (raw_data_item_match full_perm))
     (R.pts_to a full_perm c' `star`
-      raw_data_item_match c' v');
+      raw_data_item_match full_perm c' v');
   [@@inline_let]
   let res = CBOR_Case_Tagged res_tg in
   rewrite_with_implies
-    (raw_data_item_match (CBOR_Case_Tagged res_tg) (Cbor.Tagged tag v'))
-    (raw_data_item_match res (Cbor.Tagged tag v'));
+    (raw_data_item_match full_perm (CBOR_Case_Tagged res_tg) (Cbor.Tagged tag v'))
+    (raw_data_item_match full_perm res (Cbor.Tagged tag v'));
   implies_trans
-    (raw_data_item_match res (Cbor.Tagged tag v'))
-    (raw_data_item_match (CBOR_Case_Tagged res_tg) (Cbor.Tagged tag v'))
+    (raw_data_item_match full_perm res (Cbor.Tagged tag v'))
+    (raw_data_item_match full_perm (CBOR_Case_Tagged res_tg) (Cbor.Tagged tag v'))
     (R.pts_to a full_perm c' `star`
-      raw_data_item_match c' v');
+      raw_data_item_match full_perm c' v');
   return res
-
-#push-options "--z3rlimit 64"
-#restart-solver
-
-let read_cbor_tagged
-  #v a #vdest dest
-=
-  raw_data_item_match_get_case a;
-  match a with
-  | CBOR_Case_Tagged _ ->
-    let res = destr_cbor_tagged a in
-    implies_concl_r
-      (R.pts_to _ _ _ `star` raw_data_item_match _ _)
-      (raw_data_item_match _ _)
-      (exists_ (R.pts_to dest full_perm));
-    return res
-  | _ ->
-    let s = destr_cbor_serialized a in
-    let _ = gen_elim () in
-    let tag = CBOR.SteelST.Raw.read_argument_as_uint64 s.cbor_serialized_payload in
-    let s' = CBOR.SteelST.Raw.Read.focus_tagged s.cbor_serialized_payload in
-    let _ = gen_elim () in
-    implies_trans
-      (LPS.aparse CborST.parse_raw_data_item _ _)
-      (LPS.aparse CborST.parse_raw_data_item _ _)
-      (raw_data_item_match _ _);
-    let sz = LPS.get_parsed_size CborST.jump_raw_data_item s' in
-    let pl = read_valid_cbor_from_buffer_with_size_strong s' sz in
-    implies_trans
-      (raw_data_item_match _ _)
-      (LPS.aparse CborST.parse_raw_data_item _ _)
-      (raw_data_item_match _ _);
-    R.write dest pl;
-    intro_implies
-      (R.pts_to dest full_perm pl)
-      (exists_ (R.pts_to dest full_perm))
-      emp
-      (fun _ -> noop ());
-    [@@inline_let]
-    let res = {
-      cbor_tagged_tag = tag;
-      cbor_tagged_payload = dest;
-      footprint = pl;
-    }
-    in
-    rewrite_with_implies
-      (R.pts_to _ _ _)
-      (R.pts_to res.cbor_tagged_payload full_perm res.footprint);
-    implies_trans
-      (R.pts_to res.cbor_tagged_payload full_perm res.footprint)
-      (R.pts_to _ _ _)
-      (exists_ (R.pts_to dest full_perm));
-    rewrite_with_implies
-      (raw_data_item_match _ _)
-      (raw_data_item_match res.footprint (maybe_cbor_tagged_payload v));
-    implies_trans
-      (raw_data_item_match res.footprint (maybe_cbor_tagged_payload v))
-      (raw_data_item_match _ _)
-      (raw_data_item_match a v);
-    implies_join
-      (R.pts_to _ _ _)
-      (exists_ (R.pts_to dest full_perm))
-      (raw_data_item_match _ _)
-      (raw_data_item_match _ _);
-    implies_swap_r
-      (R.pts_to _ _ _ `star` raw_data_item_match _ _)
-      (exists_ (R.pts_to dest full_perm))
-      (raw_data_item_match _ _);
-    return res
 
 let serialize_cbor_tagged_eq
   (c: Cbor.raw_data_item { Cbor.Tagged? c })
@@ -2178,7 +2448,7 @@ let size_comp_for_tagged
   (va: Ghost.erased Cbor.raw_data_item)
   (c: cbor {CBOR_Case_Tagged? c})
 : Tot (cbor_size_comp_for va c)
-= fun sz perr ->
+= fun #p sz perr ->
     raw_data_item_match_get_case c;
     let _ : squash (Cbor.Tagged? va) = () in
     serialize_cbor_tagged_eq va;
@@ -2190,23 +2460,16 @@ let size_comp_for_tagged
     then begin
       noop ();
       elim_implies
-        (R.pts_to _ _ _ `star` raw_data_item_match _ _)
-        (raw_data_item_match _ _);
+        (raw_data_item_match p _ _)
+        (raw_data_item_match p _ _);
       return sz1
     end else begin
       noop ();
-      let pl = R.read c'.cbor_tagged_payload in
-      vpattern_rewrite_with_implies
-        (fun pl -> raw_data_item_match pl _)
-        pl;
-      let sz2 = size _ pl sz1 perr in
+      let sz2 = size _ c'.cbor_tagged_payload sz1 perr in
       let _ = gen_elim () in
       elim_implies
-        (raw_data_item_match pl _)
-        (raw_data_item_match _ _);
-      elim_implies
-        (R.pts_to _ _ _ `star` raw_data_item_match _ _)
-        (raw_data_item_match _ _);
+        (raw_data_item_match p _ _)
+        (raw_data_item_match p _ _);
       return sz2
     end
 
@@ -2221,7 +2484,7 @@ let l2r_writer_for_tagged
   (#va: Ghost.erased Cbor.raw_data_item)
   (c: cbor {CBOR_Case_Tagged? c})
 : Tot (cbor_l2r_writer_for va c)
-= fun #vout out ->
+= fun #p #vout out ->
     raw_data_item_match_get_case c;
     let _ : squash (Cbor.Tagged? va) = () in
     serialize_cbor_tagged_eq va;
@@ -2229,95 +2492,90 @@ let l2r_writer_for_tagged
     let res = CBOR.SteelST.Raw.Write.l2r_write_uint64_header Cbor.major_type_tagged c'.cbor_tagged_tag out in
     let _ = gen_elim () in
     let _ = LPS.elim_aparse_with_serializer CborST.serialize_header res in
-    let pl = R.read c'.cbor_tagged_payload in
-    vpattern_rewrite_with_implies
-      (fun pl -> raw_data_item_match pl _)
-      pl;
-    let res_pl = write _ pl out in
+    let res_pl = write _ c'.cbor_tagged_payload out in
     let _ = gen_elim () in
     let _ = LPS.elim_aparse_with_serializer CborST.serialize_raw_data_item res_pl in
     let _ = LPA.join res res_pl in
     let vres = LPS.intro_aparse_with_serializer CborST.serialize_raw_data_item va res in
     let vout' = vpattern_replace (LW.vp out) in
     elim_implies
-      (raw_data_item_match pl _)
-      (raw_data_item_match _ _);
-    elim_implies
-      (R.pts_to _ _ _ `star` raw_data_item_match _ _)
-      (raw_data_item_match _ _);
-    assert_ (cbor_l2r_writer_for_post va c vout out res vres vout'); // FIXME: WHY WHY WHY?
+      (raw_data_item_match p _ _)
+      (raw_data_item_match p _ _);
+    assert_ (cbor_l2r_writer_for_post p va c vout out res vres vout'); // FIXME: WHY WHY WHY?
     return res
 
 let destr_cbor_map
+  (#p: perm)
   (#v: Ghost.erased Cbor.raw_data_item)
   (a: cbor)
 : ST cbor_map
-    (raw_data_item_match a v)
+    (raw_data_item_match p a v)
     (fun res ->
-      A.pts_to res.cbor_map_payload full_perm res.footprint `star`
-      LPS.seq_list_match res.footprint (maybe_cbor_map v) (raw_data_item_map_entry_match) `star`
-      ((A.pts_to res.cbor_map_payload full_perm res.footprint `star`
-        LPS.seq_list_match res.footprint (maybe_cbor_map v) (raw_data_item_map_entry_match)) `implies_`
-        raw_data_item_match a v
+      A.pts_to res.cbor_map_payload p res.footprint `star`
+      LPS.seq_list_match res.footprint (maybe_cbor_map v) (raw_data_item_map_entry_match p) `star`
+      ((A.pts_to res.cbor_map_payload p res.footprint `star`
+        LPS.seq_list_match res.footprint (maybe_cbor_map v) (raw_data_item_map_entry_match p)) `implies_`
+        raw_data_item_match p a v
       )
     )
     (CBOR_Case_Map? a)
     (fun res ->
-      a == CBOR_Case_Map res /\
       Cbor.Map? v /\
       U64.v res.cbor_map_length == List.Tot.length (Cbor.Map?.v v)
     )
 = raw_data_item_match_get_case _;
   let sq : squash (Cbor.Map? v) = () in
-  let CBOR_Case_Map res = a in
+  let CBOR_Case_Map res fp = a in
   rewrite_with_implies
-    (raw_data_item_match _ _)
-    (raw_data_item_match (CBOR_Case_Map res) (Cbor.Map (maybe_cbor_map v)));
+    (raw_data_item_match p _ _)
+    (raw_data_item_match p (CBOR_Case_Map res fp) (Cbor.Map (maybe_cbor_map v)));
   rewrite_with_implies_with_tactic
-    (raw_data_item_match (CBOR_Case_Map res) (Cbor.Map (maybe_cbor_map v)))
-    (raw_data_item_match_map0 (CBOR_Case_Map res) (Cbor.Map (maybe_cbor_map v)) raw_data_item_map_match');
+    (raw_data_item_match p (CBOR_Case_Map res fp) (Cbor.Map (maybe_cbor_map v)))
+    (raw_data_item_match_map0 p (CBOR_Case_Map res fp) (Cbor.Map (maybe_cbor_map v)) (raw_data_item_map_match' p));
   implies_trans
-    (raw_data_item_match_map0 (CBOR_Case_Map res) (Cbor.Map (maybe_cbor_map v)) raw_data_item_map_match')
-    (raw_data_item_match (CBOR_Case_Map res) (Cbor.Map (maybe_cbor_map v)))
-    (raw_data_item_match _ _);
+    (raw_data_item_match_map0 p (CBOR_Case_Map res fp) (Cbor.Map (maybe_cbor_map v)) (raw_data_item_map_match' p))
+    (raw_data_item_match p (CBOR_Case_Map res fp) (Cbor.Map (maybe_cbor_map v)))
+    (raw_data_item_match p _ _);
   let _ = gen_elim () in
   rewrite
     (A.pts_to _ _ _)
-    (A.pts_to res.cbor_map_payload full_perm res.footprint);
+    (A.pts_to res.cbor_map_payload p res.footprint);
   rewrite
-    (raw_data_item_map_match' _ _)
-    (raw_data_item_map_match' res.footprint (maybe_cbor_map v));
+    (raw_data_item_map_match' p _ _)
+    (raw_data_item_map_match' p res.footprint (maybe_cbor_map v));
   rewrite_with_tactic
-    (raw_data_item_map_match' res.footprint (maybe_cbor_map v))
-    (LPS.seq_list_match res.footprint (maybe_cbor_map v) (raw_data_item_map_entry_match' (maybe_cbor_map v) raw_data_item_match));
-  LPS.seq_list_match_weaken res.footprint (maybe_cbor_map v) (raw_data_item_map_entry_match' (maybe_cbor_map v) raw_data_item_match) raw_data_item_map_entry_match
+    (raw_data_item_map_match' p res.footprint (maybe_cbor_map v))
+    (LPS.seq_list_match res.footprint (maybe_cbor_map v) (raw_data_item_map_entry_match' (maybe_cbor_map v) (raw_data_item_match p)));
+  LPS.seq_list_match_weaken res.footprint (maybe_cbor_map v) (raw_data_item_map_entry_match' (maybe_cbor_map v) (raw_data_item_match p)) (raw_data_item_map_entry_match p)
     (fun x y ->
       rewrite
-        (raw_data_item_map_entry_match' (maybe_cbor_map v) raw_data_item_match x y)
-        (raw_data_item_map_entry_match x y)
+        (raw_data_item_map_entry_match' (maybe_cbor_map v) (raw_data_item_match p) x y)
+        (raw_data_item_map_entry_match p x y)
     );
   intro_implies
-    (A.pts_to res.cbor_map_payload full_perm res.footprint `star`
-      LPS.seq_list_match res.footprint (maybe_cbor_map v) (raw_data_item_map_entry_match))
-    (raw_data_item_match a v)
-    (raw_data_item_match_map0 (CBOR_Case_Map res) (Cbor.Map (maybe_cbor_map v)) raw_data_item_map_match' `implies_`
-      raw_data_item_match a v)
+    (A.pts_to res.cbor_map_payload p res.footprint `star`
+      LPS.seq_list_match res.footprint (maybe_cbor_map v) (raw_data_item_map_entry_match p))
+    (raw_data_item_match p a v)
+    (GR.pts_to _ p () `star`
+      (raw_data_item_match_map0 p (CBOR_Case_Map res fp) (Cbor.Map (maybe_cbor_map v)) (raw_data_item_map_match' p) `implies_`
+        raw_data_item_match p a v)
+    )
     (fun _ ->
-      LPS.seq_list_match_weaken res.footprint (maybe_cbor_map v) raw_data_item_map_entry_match (raw_data_item_map_entry_match' (maybe_cbor_map v) raw_data_item_match)
+      LPS.seq_list_match_weaken res.footprint (maybe_cbor_map v) (raw_data_item_map_entry_match p) (raw_data_item_map_entry_match' (maybe_cbor_map v) (raw_data_item_match p))
         (fun x y ->
           rewrite
-            (raw_data_item_map_entry_match x y)
-            (raw_data_item_map_entry_match' (maybe_cbor_map v) raw_data_item_match x y)
+            (raw_data_item_map_entry_match p x y)
+            (raw_data_item_map_entry_match' (maybe_cbor_map v) (raw_data_item_match p) x y)
         );
       rewrite_with_tactic
-        (LPS.seq_list_match res.footprint (maybe_cbor_map v) (raw_data_item_map_entry_match' (maybe_cbor_map v) raw_data_item_match))
-        (raw_data_item_map_match' res.footprint (maybe_cbor_map v));
+        (LPS.seq_list_match res.footprint (maybe_cbor_map v) (raw_data_item_map_entry_match' (maybe_cbor_map v) (raw_data_item_match p)))
+        (raw_data_item_map_match' p res.footprint (maybe_cbor_map v));
       rewrite
-        (raw_data_item_map_match' res.footprint (maybe_cbor_map v)) 
-        (raw_data_item_map_match' res.footprint (Cbor.Map?.v (Cbor.Map (maybe_cbor_map v))));
+        (raw_data_item_map_match' p res.footprint (maybe_cbor_map v)) 
+        (raw_data_item_map_match' p res.footprint (Cbor.Map?.v (Cbor.Map (maybe_cbor_map v))));
       elim_implies
-        (raw_data_item_match_map0 _ _ raw_data_item_map_match')
-        (raw_data_item_match a v)
+        (raw_data_item_match_map0 p _ _ (raw_data_item_map_match' p))
+        (raw_data_item_match p a v)
     );
   return res
 
@@ -2331,16 +2589,17 @@ let size_comp_for_map_entry
     (c: cbor) ->
     cbor_size_comp_for va c
   )
+  (#p: perm)
   (va: Ghost.erased (Cbor.raw_data_item & Cbor.raw_data_item))
   (c: cbor_map_entry)
   (sz: SZ.t)
   (perr: R.ref bool)
 : STT SZ.t
-    (raw_data_item_map_entry_match c (Ghost.reveal va) `star`
+    (raw_data_item_map_entry_match p c (Ghost.reveal va) `star`
       R.pts_to perr full_perm false
     )
     (fun res ->
-      raw_data_item_map_entry_match c (Ghost.reveal va) `star`
+      raw_data_item_map_entry_match p c (Ghost.reveal va) `star`
       exists_ (fun err ->
         R.pts_to perr full_perm err `star`
         pure (LowParse.SteelST.Write.size_comp_for_post (LPS.serialize_nondep_then CborST.serialize_raw_data_item CborST.serialize_raw_data_item) va sz res err)
@@ -2371,54 +2630,56 @@ let constr_cbor_map
     footprint = c';
   }
   in
+  let fp = GR.alloc () in
   [@@inline_let]
-  let res = CBOR_Case_Map ares in
+  let res = CBOR_Case_Map ares fp in
   noop ();
   SM.seq_list_match_weaken
     c' v'
-    raw_data_item_map_entry_match
-    (raw_data_item_map_entry_match' v' raw_data_item_match)
+    (raw_data_item_map_entry_match full_perm)
+    (raw_data_item_map_entry_match' v' (raw_data_item_match full_perm))
     (fun x y ->
       rewrite
-        (raw_data_item_map_entry_match x y)
-        (raw_data_item_map_entry_match' v' raw_data_item_match x y)
+        (raw_data_item_map_entry_match full_perm x y)
+        (raw_data_item_map_entry_match' v' (raw_data_item_match full_perm) x y)
     );
   rewrite_with_implies_with_tactic
-    (raw_data_item_match_map0 (CBOR_Case_Map ares) (Cbor.Map v') raw_data_item_map_match')
-    (raw_data_item_match (CBOR_Case_Map ares) (Cbor.Map v'));
+    (raw_data_item_match_map0 full_perm (CBOR_Case_Map ares fp) (Cbor.Map v') (raw_data_item_map_match' full_perm))
+    (raw_data_item_match full_perm (CBOR_Case_Map ares fp) (Cbor.Map v'));
   rewrite_with_implies
-    (raw_data_item_match (CBOR_Case_Map ares) (Cbor.Map v'))
-    (raw_data_item_match res (Cbor.Map v'));
+    (raw_data_item_match full_perm (CBOR_Case_Map ares fp) (Cbor.Map v'))
+    (raw_data_item_match full_perm res (Cbor.Map v'));
   implies_trans
-    (raw_data_item_match res (Cbor.Map v'))
-    (raw_data_item_match (CBOR_Case_Map ares) (Cbor.Map v'))
-    (raw_data_item_match_map0 (CBOR_Case_Map ares) (Cbor.Map v') raw_data_item_map_match');
+    (raw_data_item_match full_perm res (Cbor.Map v'))
+    (raw_data_item_match full_perm (CBOR_Case_Map ares fp) (Cbor.Map v'))
+    (raw_data_item_match_map0 full_perm (CBOR_Case_Map ares fp) (Cbor.Map v') (raw_data_item_map_match' full_perm));
   intro_implies
-    (raw_data_item_match_map0 (CBOR_Case_Map ares) (Cbor.Map v') raw_data_item_map_match')
-    (A.pts_to a full_perm c' `star` raw_data_item_map_match c' v')
+    (raw_data_item_match_map0 full_perm (CBOR_Case_Map ares fp) (Cbor.Map v') (raw_data_item_map_match' full_perm))
+    (A.pts_to a full_perm c' `star` raw_data_item_map_match full_perm c' v')
     emp
     (fun _ ->
       let _ = gen_elim () in
+      GR.free _;
       rewrite
         (A.pts_to _ _ _)
         (A.pts_to a full_perm c');
       rewrite
-        (raw_data_item_map_match' _ _)
-        (raw_data_item_map_match' c' v');
+        (raw_data_item_map_match' full_perm _ _)
+        (raw_data_item_map_match' full_perm c' v');
       SM.seq_list_match_weaken
         c' v'
-        (raw_data_item_map_entry_match' v' raw_data_item_match)
-        raw_data_item_map_entry_match
+        (raw_data_item_map_entry_match' v' (raw_data_item_match full_perm))
+        (raw_data_item_map_entry_match full_perm)
         (fun x y ->
           rewrite
-            (raw_data_item_map_entry_match' v' raw_data_item_match x y)
-            (raw_data_item_map_entry_match x y)
+            (raw_data_item_map_entry_match' v' (raw_data_item_match full_perm) x y)
+            (raw_data_item_map_entry_match full_perm x y)
         )
     );
   implies_trans
-    (raw_data_item_match res (Cbor.Map v'))
-    (raw_data_item_match_map0 (CBOR_Case_Map ares) (Cbor.Map v') raw_data_item_map_match')
-    (A.pts_to a full_perm c' `star` raw_data_item_map_match c' v');
+    (raw_data_item_match full_perm res (Cbor.Map v'))
+    (raw_data_item_match_map0 full_perm (CBOR_Case_Map ares fp) (Cbor.Map v') (raw_data_item_map_match' full_perm))
+    (A.pts_to a full_perm c' `star` raw_data_item_map_match full_perm c' v');
   return res
 
 #push-options "--z3rlimit 64"
@@ -2454,7 +2715,7 @@ let size_comp_for_map
   (va: Ghost.erased Cbor.raw_data_item)
   (c: cbor {CBOR_Case_Map? c})
 : Tot (cbor_size_comp_for va c)
-= fun sz perr ->
+= fun #p sz perr ->
     let _ = A.intro_fits_u64 () in
     raw_data_item_match_get_case c;
     let _ : squash (Cbor.Map? va) = () in
@@ -2463,14 +2724,14 @@ let size_comp_for_map
     let l = Ghost.hide (maybe_cbor_map va) in
     assert (Ghost.reveal l == Cbor.Map?.v va);
     rewrite_with_implies
-      (LPS.seq_list_match c'.footprint _ (raw_data_item_map_entry_match))
-      (LPS.seq_list_match c'.footprint l (raw_data_item_map_entry_match));
+      (LPS.seq_list_match c'.footprint _ (raw_data_item_map_entry_match p))
+      (LPS.seq_list_match c'.footprint l (raw_data_item_map_entry_match p));
     implies_trans_r1
       (A.pts_to _ _ _)
-      (LPS.seq_list_match c'.footprint l (raw_data_item_map_entry_match))
-      (LPS.seq_list_match c'.footprint _ (raw_data_item_map_entry_match))
-      (raw_data_item_match _ _);
-    LPS.seq_list_match_length (raw_data_item_map_entry_match) _ _;
+      (LPS.seq_list_match c'.footprint l (raw_data_item_map_entry_match p))
+      (LPS.seq_list_match c'.footprint _ (raw_data_item_map_entry_match p))
+      (raw_data_item_match p _ _);
+    LPS.seq_list_match_length (raw_data_item_map_entry_match p) _ _;
     A.pts_to_length _ _;
     let sz1 = CBOR.SteelST.Raw.Write.size_comp_uint64_header Cbor.major_type_map c'.cbor_map_length sz perr in
     let _ = gen_elim () in
@@ -2479,14 +2740,14 @@ let size_comp_for_map
     then begin
       noop ();
       elim_implies
-        (A.pts_to _ _ _ `star` LPS.seq_list_match c'.footprint l (raw_data_item_map_entry_match))
-        (raw_data_item_match _ _);
+        (A.pts_to _ _ _ `star` LPS.seq_list_match c'.footprint l (raw_data_item_map_entry_match p))
+        (raw_data_item_match p _ _);
       return sz1
     end else begin
       noop ();
       let sz2 = LPS.array_payload_as_nlist_size
         (LPS.serialize_nondep_then CborST.serialize_raw_data_item CborST.serialize_raw_data_item)
-        (raw_data_item_map_entry_match)
+        (raw_data_item_map_entry_match p)
         (fun x y sz perr ->
           let res = size_comp_for_map_entry size y x sz perr in
           let _ = gen_elim () in
@@ -2501,8 +2762,8 @@ let size_comp_for_map
       in
       let _ = gen_elim () in
       elim_implies
-        (A.pts_to _ _ _ `star` LPS.seq_list_match c'.footprint l (raw_data_item_map_entry_match))
-        (raw_data_item_match _ _);
+        (A.pts_to _ _ _ `star` LPS.seq_list_match c'.footprint l (raw_data_item_map_entry_match p))
+        (raw_data_item_match p _ _);
       return sz2
     end
 
@@ -2520,6 +2781,7 @@ let l2r_write_map_entry_post
 
 [@@__reduce__]
 let l2r_writer_for_map_entry_post
+  (p: perm)
   (va: Ghost.erased (Cbor.raw_data_item & Cbor.raw_data_item))
   (c: cbor_map_entry)
   (vout: LPA.array LPS.byte)
@@ -2529,7 +2791,7 @@ let l2r_writer_for_map_entry_post
   (vout': LPA.array LPS.byte)
 : Tot vprop
 =
-  raw_data_item_map_entry_match c (Ghost.reveal va) `star`
+  raw_data_item_map_entry_match p c (Ghost.reveal va) `star`
   LPS.aparse (LPS.nondep_then CborST.parse_raw_data_item CborST.parse_raw_data_item) res vres `star`
   LW.vp out vout' `star`
   pure (
@@ -2546,14 +2808,15 @@ let l2r_writer_for_map_entry
   )
   (va: Ghost.erased (Cbor.raw_data_item & Cbor.raw_data_item))
   (c: cbor_map_entry)
+  (#p: perm)
   (#vout: LPA.array LPS.byte)
   (out: LW.t)
 : ST LPS.byte_array
-    (raw_data_item_map_entry_match c (Ghost.reveal va) `star`
+    (raw_data_item_map_entry_match p c (Ghost.reveal va) `star`
       LW.vp out vout
     )
     (fun res -> exists_ (fun vres -> exists_ (fun vout' ->
-      l2r_writer_for_map_entry_post va c vout out res vres vout'
+      l2r_writer_for_map_entry_post p va c vout out res vres vout'
     )))
     (Seq.length (LPS.serialize (LPS.serialize_nondep_then CborST.serialize_raw_data_item CborST.serialize_raw_data_item) va) <= LPA.length vout)
     (fun _ -> True)
@@ -2568,7 +2831,7 @@ let l2r_writer_for_map_entry
   let _ = LPS.elim_aparse_with_serializer CborST.serialize_raw_data_item res_pl in
   let _ = LPA.join res res_pl in
   let vres = LPS.intro_aparse_with_serializer (LPS.serialize_nondep_then CborST.serialize_raw_data_item CborST.serialize_raw_data_item) va res in
-  assert_ (l2r_writer_for_map_entry_post va c vout out res vres vout');
+  assert_ (l2r_writer_for_map_entry_post p va c vout out res vres vout');
   return res
 
 inline_for_extraction
@@ -2582,7 +2845,7 @@ let l2r_writer_for_map
   (va: Ghost.erased Cbor.raw_data_item)
   (c: cbor {CBOR_Case_Map? c})
 : Tot (cbor_l2r_writer_for va c)
-= fun #vout out ->
+= fun #p #vout out ->
     let _ = A.intro_fits_u64 () in
     raw_data_item_match_get_case c;
     let _ : squash (Cbor.Map? va) = () in
@@ -2591,21 +2854,21 @@ let l2r_writer_for_map
     let l = Ghost.hide (maybe_cbor_map va) in
     assert (Ghost.reveal l == Cbor.Map?.v va);
     rewrite_with_implies
-      (LPS.seq_list_match c'.footprint _ (raw_data_item_map_entry_match))
-      (LPS.seq_list_match c'.footprint l (raw_data_item_map_entry_match));
+      (LPS.seq_list_match c'.footprint _ (raw_data_item_map_entry_match p))
+      (LPS.seq_list_match c'.footprint l (raw_data_item_map_entry_match p));
     implies_trans_r1
       (A.pts_to _ _ _)
-      (LPS.seq_list_match c'.footprint l (raw_data_item_map_entry_match))
-      (LPS.seq_list_match c'.footprint _ (raw_data_item_map_entry_match))
-      (raw_data_item_match _ _);
-    LPS.seq_list_match_length (raw_data_item_map_entry_match) _ _;
+      (LPS.seq_list_match c'.footprint l (raw_data_item_map_entry_match p))
+      (LPS.seq_list_match c'.footprint _ (raw_data_item_map_entry_match p))
+      (raw_data_item_match p _ _);
+    LPS.seq_list_match_length (raw_data_item_map_entry_match p) _ _;
     A.pts_to_length _ _;
     let res = CBOR.SteelST.Raw.Write.l2r_write_uint64_header Cbor.major_type_map c'.cbor_map_length out in
     let _ = gen_elim () in
     let _ = LPS.elim_aparse_with_serializer CborST.serialize_header res in
     let res_pl = LPS.l2r_write_array_payload_as_nlist
       (LPS.serialize_nondep_then CborST.serialize_raw_data_item CborST.serialize_raw_data_item)
-      (raw_data_item_map_entry_match)
+      (raw_data_item_map_entry_match p)
       (fun x y out ->
          let res = l2r_writer_for_map_entry write y x out in
          let _ = gen_elim () in
@@ -2624,46 +2887,46 @@ let l2r_writer_for_map
     let _ = gen_elim () in
     let vres = LPS.intro_aparse_with_serializer CborST.serialize_raw_data_item va res in
     elim_implies
-      (A.pts_to _ _ _ `star` LPS.seq_list_match c'.footprint l (raw_data_item_map_entry_match))
-      (raw_data_item_match _ _);
-    assert_ (cbor_l2r_writer_for_post va c vout out res vres vout'); // FIXME: WHY WHY WHY?
+      (A.pts_to _ _ _ `star` LPS.seq_list_match c'.footprint l (raw_data_item_map_entry_match p))
+      (raw_data_item_match p _ _);
+    assert_ (cbor_l2r_writer_for_post p va c vout out res vres vout'); // FIXME: WHY WHY WHY?
     return res
 
 #pop-options
 
 let cbor_get_major_type
-  #v a
+  #p #v a
 = raw_data_item_match_get_case a;
   match a with
-  | CBOR_Case_Map _ ->
+  | CBOR_Case_Map _ _ ->
     noop ();
     return Cbor.major_type_map
-  | CBOR_Case_Array _ ->
+  | CBOR_Case_Array _ _ ->
     noop ();
     return Cbor.major_type_array
   | CBOR_Case_Tagged _ ->
     noop ();
     return Cbor.major_type_tagged
-  | CBOR_Case_Simple_value _ ->
+  | CBOR_Case_Simple_value _ _ ->
     noop ();
     return Cbor.major_type_simple_value
-  | CBOR_Case_String _ ->
+  | CBOR_Case_String _ _ _ ->
     let s = destr_cbor_string a in
     let _ = gen_elim () in
-    elim_implies (A.pts_to _ _ _) (raw_data_item_match _ _);
+    elim_implies (A.pts_to _ _ _) (raw_data_item_match p _ _);
     return s.cbor_string_type
-  | CBOR_Case_Int64 _ ->
+  | CBOR_Case_Int64 _ _ ->
     let i = destr_cbor_int64 a in
     return i.cbor_int_type
   | _ ->
     let s = destr_cbor_serialized a in
     let _ = gen_elim () in
     let res = CborST.read_major_type s.cbor_serialized_payload in
-    elim_implies (LPS.aparse CborST.parse_raw_data_item _ _) (raw_data_item_match _ _);
+    elim_implies (LPS.aparse CborST.parse_raw_data_item _ _) (raw_data_item_match p _ _);
     return res
 
 let cbor_is_equal
-  #v1 a1 #v2 a2
+  #p1 #v1 a1 #p2 #v2 a2
 =
   let _ = A.intro_fits_u64 () in
   let type1 = cbor_get_major_type a1 in
@@ -2699,8 +2962,8 @@ let cbor_is_equal
       let res = LowParse.SteelST.Assoc.eq_byte_arrays t1 (SZ.uint64_to_sizet s1.cbor_string_length) t2 (SZ.uint64_to_sizet s2.cbor_string_length) in
       elim_implies (LPA.arrayptr t1 _) (A.pts_to _ _ _);
       elim_implies (LPA.arrayptr t2 _) (A.pts_to _ _ _);
-      elim_implies (A.pts_to s1.cbor_string_payload _ _) (raw_data_item_match _ _);
-      elim_implies (A.pts_to s2.cbor_string_payload _ _) (raw_data_item_match _ _);
+      elim_implies (A.pts_to s1.cbor_string_payload _ _) (raw_data_item_match p1 _ _);
+      elim_implies (A.pts_to s2.cbor_string_payload _ _) (raw_data_item_match p2 _ _);
       return res
     end
     else begin
@@ -2711,48 +2974,54 @@ let cbor_is_equal
   end
 
 assume val cbor_map_get_case_map
+  (#pkey: perm)
   (#vkey: Ghost.erased Cbor.raw_data_item)
   (key: cbor)
+  (#pmap: perm)
   (#vmap: Ghost.erased Cbor.raw_data_item)
   (map: cbor { Cbor.Map? vmap })
 : ST cbor_map_get_t
-    (raw_data_item_match key vkey `star` raw_data_item_match map vmap)
-    (fun res -> raw_data_item_match key vkey `star` cbor_map_get_post vkey vmap map res)
+    (raw_data_item_match pkey key vkey `star` raw_data_item_match pmap map vmap)
+    (fun res -> raw_data_item_match pkey key vkey `star` cbor_map_get_post pmap vkey vmap map res)
     (~ (Cbor.Tagged? vkey \/ Cbor.Array? vkey \/ Cbor.Map? vkey) /\
       CBOR_Case_Map? map
     )
     (fun res -> Found? res == Some? (Cbor.list_ghost_assoc (Ghost.reveal vkey) (Cbor.Map?.v vmap)))
 
 let mk_cbor_nlist_assoc_eq_keys
+  (pkey: perm)
   (vkey: Ghost.erased Cbor.raw_data_item)
   (key: cbor {
     ~ (Cbor.Tagged? vkey \/ Cbor.Array? vkey \/ Cbor.Map? vkey)
   })
-: Tot (LowParse.SteelST.Assoc.nlist_assoc_eq_keys CborST.parse_raw_data_item (Ghost.reveal vkey) (raw_data_item_match key vkey))
+: Tot (LowParse.SteelST.Assoc.nlist_assoc_eq_keys CborST.parse_raw_data_item (Ghost.reveal vkey) (raw_data_item_match pkey key vkey))
 = fun #va a sz ->
-    let x = read_valid_cbor_from_buffer_with_size_strong a sz in
+    let x = read_valid_cbor_from_buffer_with_size_strong full_perm a sz in
     let res = cbor_is_equal key x in
     elim_implies
-      (raw_data_item_match x _)
+      (raw_data_item_match full_perm x _)
       (LPS.aparse CborST.parse_raw_data_item _ _);
     return res
 
 let cbor_map_get_case_serialized
+  (#pkey: perm)
   (#vkey: Ghost.erased Cbor.raw_data_item)
   (key: cbor)
+  (#pmap: perm)
   (#vmap: Ghost.erased Cbor.raw_data_item)
   (map: cbor { Cbor.Map? vmap })
 : ST cbor_map_get_t
-    (raw_data_item_match key vkey `star` raw_data_item_match map vmap)
+    (raw_data_item_match pkey key vkey `star` raw_data_item_match pmap map vmap)
     (fun res ->
-      raw_data_item_match key vkey `star` cbor_map_get_post vkey vmap map res `star` 
+      raw_data_item_match pkey key vkey `star` cbor_map_get_post pmap vkey vmap map res `star` 
       pure (Found? res == Some? (Cbor.list_ghost_assoc (Ghost.reveal vkey) (Cbor.Map?.v vmap)))
     )
     (~ (Cbor.Tagged? vkey \/ Cbor.Array? vkey \/ Cbor.Map? vkey) /\
       CBOR_Case_Serialized? map
     )
     (fun _ -> True)
-= let _ = A.intro_fits_u64 () in
+= raw_data_item_match_perm_le_full_perm map;
+  let _ = A.intro_fits_u64 () in
   let s = destr_cbor_serialized map in
   let _ = gen_elim () in
   let len64 = CborST.read_argument_as_uint64 s.cbor_serialized_payload in
@@ -2762,7 +3031,7 @@ let cbor_map_get_case_serialized
   implies_trans
     (LPS.aparse (LPS.parse_nlist (SZ.v len) (LPS.nondep_then CborST.parse_raw_data_item CborST.parse_raw_data_item)) _ _)
     (LPS.aparse CborST.parse_raw_data_item _ _)
-    (raw_data_item_match map vmap);
+    (raw_data_item_match pmap map vmap);
   let vm = vpattern (LPS.aparse (LPS.parse_nlist (SZ.v len) (LPS.nondep_then CborST.parse_raw_data_item CborST.parse_raw_data_item)) _) in
   vpattern_rewrite_with_implies
     (LPS.aparse (LPS.parse_nlist (SZ.v len) (LPS.nondep_then CborST.parse_raw_data_item CborST.parse_raw_data_item)) _)
@@ -2770,15 +3039,15 @@ let cbor_map_get_case_serialized
   implies_trans
     (LPS.aparse (LPS.parse_nlist (SZ.v len) (LPS.nondep_then CborST.parse_raw_data_item CborST.parse_raw_data_item)) _ _)
     (LPS.aparse (LPS.parse_nlist (SZ.v len) (LPS.nondep_then CborST.parse_raw_data_item CborST.parse_raw_data_item)) _ _)
-    (raw_data_item_match map vmap);
+    (raw_data_item_match pmap map vmap);
   R.with_local m (fun pa ->
     noop ();
     let found = LowParse.SteelST.Assoc.nlist_assoc
       CborST.jump_raw_data_item
       CborST.jump_raw_data_item
       #vkey
-      #(raw_data_item_match key vkey)
-      (mk_cbor_nlist_assoc_eq_keys vkey key)
+      #(raw_data_item_match pkey key vkey)
+      (mk_cbor_nlist_assoc_eq_keys pkey vkey key)
       len
       m
       pa
@@ -2787,13 +3056,13 @@ let cbor_map_get_case_serialized
     then begin
       noop ();
       rewrite
-        (LowParse.SteelST.Assoc.nlist_assoc_post CborST.parse_raw_data_item CborST.parse_raw_data_item vkey (raw_data_item_match key vkey) (SZ.v len) vm m pa found)
-        (LowParse.SteelST.Assoc.nlist_assoc_post_success CborST.parse_raw_data_item CborST.parse_raw_data_item vkey (raw_data_item_match key vkey) (SZ.v len) vm m pa);
+        (LowParse.SteelST.Assoc.nlist_assoc_post CborST.parse_raw_data_item CborST.parse_raw_data_item vkey (raw_data_item_match pkey key vkey) (SZ.v len) vm m pa found)
+        (LowParse.SteelST.Assoc.nlist_assoc_post_success CborST.parse_raw_data_item CborST.parse_raw_data_item vkey (raw_data_item_match pkey key vkey) (SZ.v len) vm m pa);
       let _ = gen_elim () in
       implies_trans
         (LPS.aparse CborST.parse_raw_data_item _ _)
         (LPS.aparse (LPS.parse_nlist (SZ.v len) (LPS.nondep_then CborST.parse_raw_data_item CborST.parse_raw_data_item)) _ _)
-        (raw_data_item_match map vmap);
+        (raw_data_item_match pmap map vmap);
       let a = R.read pa in
       vpattern_rewrite_with_implies
         (fun a -> LPS.aparse CborST.parse_raw_data_item a _)
@@ -2801,38 +3070,38 @@ let cbor_map_get_case_serialized
       implies_trans
         (LPS.aparse CborST.parse_raw_data_item _ _)
         (LPS.aparse CborST.parse_raw_data_item _ _)
-        (raw_data_item_match map vmap);
+        (raw_data_item_match pmap map vmap);
       let sz = LPS.get_parsed_size CborST.jump_raw_data_item a in
-      let res_succ = read_valid_cbor_from_buffer_with_size_strong a sz in
+      let res_succ = read_valid_cbor_from_buffer_with_size_strong pmap a sz in
       implies_trans
-        (raw_data_item_match res_succ _)
+        (raw_data_item_match pmap res_succ _)
         (LPS.aparse CborST.parse_raw_data_item _ _)
-        (raw_data_item_match map vmap);
+        (raw_data_item_match pmap map vmap);
       rewrite
-        (cbor_map_get_post_found vkey vmap map res_succ)
-        (cbor_map_get_post vkey vmap map (Found res_succ));
+        (cbor_map_get_post_found pmap vkey vmap map res_succ)
+        (cbor_map_get_post pmap vkey vmap map (Found res_succ));
       return (Found res_succ)
     end else begin
       noop ();
       rewrite
-        (LowParse.SteelST.Assoc.nlist_assoc_post CborST.parse_raw_data_item CborST.parse_raw_data_item vkey (raw_data_item_match key vkey) (SZ.v len) vm m pa found)
-        (LowParse.SteelST.Assoc.nlist_assoc_post_failure CborST.parse_raw_data_item CborST.parse_raw_data_item vkey (raw_data_item_match key vkey) (SZ.v len) vm m pa);
+        (LowParse.SteelST.Assoc.nlist_assoc_post CborST.parse_raw_data_item CborST.parse_raw_data_item vkey (raw_data_item_match pkey key vkey) (SZ.v len) vm m pa found)
+        (LowParse.SteelST.Assoc.nlist_assoc_post_failure CborST.parse_raw_data_item CborST.parse_raw_data_item vkey (raw_data_item_match pkey key vkey) (SZ.v len) vm m pa);
       let _ = gen_elim () in
       elim_implies
         (LPS.aparse (LPS.parse_nlist (SZ.v len) (LPS.nondep_then CborST.parse_raw_data_item CborST.parse_raw_data_item)) _ _)
-        (raw_data_item_match map vmap);
+        (raw_data_item_match pmap map vmap);
       rewrite
-        (cbor_map_get_post_not_found vkey vmap map)
-        (cbor_map_get_post vkey vmap map NotFound);
+        (cbor_map_get_post_not_found pmap vkey vmap map)
+        (cbor_map_get_post pmap vkey vmap map NotFound);
       return NotFound
     end
   )
 
 let cbor_map_get
-  #vkey key #vmap map
+  key map
 = raw_data_item_match_get_case map;
   match map with
-  | CBOR_Case_Map _ ->
+  | CBOR_Case_Map _ _ ->
     let res = cbor_map_get_case_map key map in
     return res
   | _ ->
@@ -2843,14 +3112,15 @@ let cbor_map_get
 let rec cbor_size_comp
   (va: Ghost.erased Cbor.raw_data_item)
   (c: cbor)
+  (#p: perm)
   (sz: SZ.t)
   (perr: R.ref bool)
 : STT SZ.t // FIXME: WHY WHY WHY do I need to expand the type annotation to avoid the termination check?
-    (raw_data_item_match c (Ghost.reveal va) `star`
+    (raw_data_item_match p c (Ghost.reveal va) `star`
       R.pts_to perr full_perm false
     )
     (fun res ->
-      raw_data_item_match c (Ghost.reveal va) `star`
+      raw_data_item_match p c (Ghost.reveal va) `star`
       exists_ (fun err ->
         R.pts_to perr full_perm err `star`
         pure (LowParse.SteelST.Write.size_comp_for_post CborST.serialize_raw_data_item va sz res err)
@@ -2858,51 +3128,53 @@ let rec cbor_size_comp
 =
   raw_data_item_match_get_case c;
   match c with
-  | CBOR_Case_Int64 _ -> size_comp_for_int64 va c sz perr
-  | CBOR_Case_Simple_value _ -> size_comp_for_simple_value va c sz perr
-  | CBOR_Case_String _ -> size_comp_for_string va c sz perr
+  | CBOR_Case_Int64 _ _ -> size_comp_for_int64 va c sz perr
+  | CBOR_Case_Simple_value _ _ -> size_comp_for_simple_value va c sz perr
+  | CBOR_Case_String _ _ _ -> size_comp_for_string va c sz perr
   | CBOR_Case_Tagged _ -> size_comp_for_tagged cbor_size_comp va c sz perr
-  | CBOR_Case_Array _ -> size_comp_for_array cbor_size_comp va c sz perr
-  | CBOR_Case_Map _ -> size_comp_for_map cbor_size_comp va c sz perr
+  | CBOR_Case_Array _ _ -> size_comp_for_array cbor_size_comp va c sz perr
+  | CBOR_Case_Map _ _ -> size_comp_for_map cbor_size_comp va c sz perr
   | _ -> size_comp_for_serialized c sz perr
 
 let rec cbor_l2r_write
   (va: Ghost.erased Cbor.raw_data_item)
   (c: cbor)
+  (#p: perm)
   (#vout: LPA.array LPS.byte)
   (out: LW.t)
 : ST LPS.byte_array // FIXME: WHY WHY WHY do I need to expand the type annotation to avoid the termination check?
-    (raw_data_item_match c (Ghost.reveal va) `star`
+    (raw_data_item_match p c (Ghost.reveal va) `star`
       LW.vp out vout
     )
     (fun res -> exists_ (fun (vres: LPS.v CborST.parse_raw_data_item_kind Cbor.raw_data_item) -> exists_ (fun (vout': LPA.array LPS.byte) ->
-      cbor_l2r_writer_for_post va c vout out res vres vout'
+      cbor_l2r_writer_for_post p va c vout out res vres vout'
     )))
     (Seq.length (LPS.serialize CborST.serialize_raw_data_item va) <= LPA.length vout)
     (fun _ -> True)
 =
   raw_data_item_match_get_case c;
   match c with
-  | CBOR_Case_Int64 _ -> l2r_writer_for_int64 va c out
-  | CBOR_Case_Simple_value _ -> l2r_writer_for_simple_value va c out
-  | CBOR_Case_String _ -> l2r_write_cbor_string va c out
+  | CBOR_Case_Int64 _ _ -> l2r_writer_for_int64 va c out
+  | CBOR_Case_Simple_value _ _ -> l2r_writer_for_simple_value va c out
+  | CBOR_Case_String _ _ _ -> l2r_write_cbor_string va c out
   | CBOR_Case_Tagged _ -> l2r_writer_for_tagged cbor_l2r_write c out
-  | CBOR_Case_Array _ -> l2r_writer_for_array cbor_l2r_write va c out
-  | CBOR_Case_Map _ -> l2r_writer_for_map cbor_l2r_write va c out
+  | CBOR_Case_Array _ _ -> l2r_writer_for_array cbor_l2r_write va c out
+  | CBOR_Case_Map _ _ -> l2r_writer_for_map cbor_l2r_write va c out
   | _ -> l2r_writer_for_serialized c out
 
 let write_cbor
+  (#p: perm)
   (#va: Ghost.erased Cbor.raw_data_item)
   (c: cbor)
   (#vout: Ghost.erased (Seq.seq U8.t))
   (out: A.array U8.t)
   (sz: SZ.t)
 : ST SZ.t
-    (raw_data_item_match c (Ghost.reveal va) `star`
+    (raw_data_item_match p c (Ghost.reveal va) `star`
       A.pts_to out full_perm vout
     )
     (fun res -> 
-      raw_data_item_match c (Ghost.reveal va) `star`
+      raw_data_item_match p c (Ghost.reveal va) `star`
       exists_ (write_cbor_post va c vout out res)
     )
     (SZ.v sz == A.length out)
